Refactoring to allow fupd in semax.
Invariants and world satisfaction are now defined in veric and don't rely on Iris. We still have the same surface rules, because any proof of a program that takes advantage of invariants will probably use Iris.

floyd/sublist.v
@@ -13,6 +13,7 @@ Instance Inhabitant_fun {T1 T2: Type} {H: Inhabitant T2} : Inhabitant (T1->T2) :
 Instance Inhabitant_Prop : Inhabitant Prop := False.
 Instance Inhabitant_bool : Inhabitant bool := false.
 Instance Inhabitant_pair {T1 T2 : Type} {x1: Inhabitant T1} {x2: Inhabitant T2} : Inhabitant (T1*T2)%type := (x1,x2).
+Instance Inhabitant_option {A} : Inhabitant (option A) := None.
 
 Lemma Zlength_length:
   forall A (al: list A) (n: Z),
@@ -1618,5 +1619,662 @@ Lemma nth_Znth {A} {d: Inhabitant A}:
 forall n (xs:list A), 0 <= n < Zlength xs -> (nth (Z.to_nat n) xs d) = (Znth n xs).
 Proof. intros; unfold Znth; if_tac; unfold default. omega. reflexivity. Qed.
 
+Lemma nth_Znth' : forall {A}{d: Inhabitant A} i l, nth i l default = Znth (Z.of_nat i) l.
+Proof.
+  intros; unfold Znth.
+  destruct (zlt (Z.of_nat i) 0); [omega|].
+  rewrite Nat2Z.id; auto.
+Qed.
 
- 
+ Lemma In_Znth : forall {A} {d: Inhabitant A} (l : list A) x,
+    In x l ->
+    exists i, 0 <= i < Zlength l /\ Znth i l = x.
+Proof.
+  unfold Znth; intros.
+  apply In_nth with (d := d) in H; destruct H as (n & ? & ?).
+  exists (Z.of_nat n); split.
+  - rewrite Zlength_correct; omega.
+  - destruct (zlt (Z.of_nat n) 0); [omega|].
+    rewrite Nat2Z.id; auto.
+Qed.
+
+Lemma In_upd_Znth_old : forall {A}{d: Inhabitant A} i (x y : A) l, In x l -> x <> Znth i l -> 0 <= i <= Zlength l ->
+  In x (upd_Znth i l y).
+Proof.
+  intros.
+  apply In_Znth in H; destruct H as (j & ? & ?); subst.
+  unfold upd_Znth.
+  destruct (Z.eq_dec j i); [subst; contradiction|].
+  rewrite in_app; simpl.
+  destruct (zlt j i); [left | right; right].
+  - erewrite <- (Z.add_0_r j), <- Znth_sublist; [apply Znth_In; rewrite Zlength_sublist| |]; auto; omega.
+  - erewrite <- (Z.sub_simpl_r _ (i + 1)), <- Znth_sublist; [apply Znth_In; rewrite Zlength_sublist| |]; omega.
+Qed.
+
+Lemma Znth_combine : forall {A B} {a: Inhabitant A} {b: Inhabitant B} i (l1: list A) (l2: list B), 
+   Zlength l1 = Zlength l2 ->
+  Znth i (combine l1 l2) = (Znth i l1, Znth i l2).
+Proof.
+  intros; unfold Znth.
+  destruct (zlt i 0); auto.
+  apply combine_nth.
+  rewrite !Zlength_correct in *; omega.
+Qed.
+
+Lemma Zlength_combine : forall {A B} (l : list A) (l' : list B),
+  Zlength (combine l l') = Z.min (Zlength l) (Zlength l').
+Proof.
+  intros; rewrite !Zlength_correct, combine_length, Nat2Z.inj_min; auto.
+Qed.
+
+Lemma upd_Znth_cons : forall {A} i a l (x : A), i > 0 ->
+  upd_Znth i (a :: l) x = a :: upd_Znth (i - 1) l x.
+Proof.
+  intros; unfold upd_Znth, sublist.sublist; simpl.
+  repeat rewrite Z.sub_0_r.
+  destruct (Z.to_nat i) eqn: Hi.
+  { apply f_equal with (f := Z.of_nat) in Hi.
+    rewrite Z2Nat.id in Hi; subst; simpl in *; omega. }
+  rewrite Zlength_cons; repeat rewrite Z2Nat.inj_add; try omega.
+  repeat rewrite Z2Nat.inj_sub; try omega.
+  rewrite Hi; simpl.
+  rewrite Nat.sub_0_r.
+  do 4 f_equal.
+  rewrite Z2Nat.inj_succ; [|rewrite Zlength_correct; omega].
+  repeat rewrite Z2Nat.inj_add; try omega.
+  rewrite Z2Nat.inj_sub; try omega.
+  change (Z.to_nat 1) with 1%nat; omega.
+Qed.
+
+Lemma sublist_next : forall {A}{d: Inhabitant A} i j l,
+      0 <= i < j -> j <= Zlength l ->
+  sublist i j l = Znth i l :: sublist (i + 1) j l.
+Proof.
+  intros.
+  rewrite Znth_cons_sublist; [|omega].
+  apply sublist_split; omega.
+Qed.
+
+Lemma upd_Znth_triv : forall {A}{d: Inhabitant A} i (l : list A) x (Hi : 0 <= i < Zlength l),
+  Znth i l = x -> upd_Znth i l x = l.
+Proof.
+  intros; unfold upd_Znth.
+  subst; rewrite <- sublist_next by omega.
+  rewrite <- sublist_split, sublist_same; auto; omega.
+Qed.
+
+Lemma combine_upd_Znth : forall {A B} (l1 : list A) (l2 : list B) i x1 x2, 0 <= i < Zlength l1 ->
+  Zlength l1 = Zlength l2 -> combine (upd_Znth i l1 x1) (upd_Znth i l2 x2) = upd_Znth i (combine l1 l2) (x1, x2).
+Proof.
+  induction l1; simpl; intros; [rewrite Zlength_nil in *; omega|].
+  destruct l2; [rewrite Zlength_nil in *; omega|].
+  rewrite !Zlength_cons in *.
+  destruct (Z.eq_dec i 0).
+  - subst; rewrite !upd_Znth0, !Zlength_cons, !sublist_1_cons, !sublist_same; auto; omega.
+  - rewrite !upd_Znth_cons; try omega; simpl.
+    rewrite IHl1; auto; omega.
+Qed.
+
+Corollary combine_upd_Znth1 : forall {A B}{d: Inhabitant B} (l1 : list A) (l2 : list B) i x,
+   0 <= i < Zlength l1 ->
+  Zlength l1 = Zlength l2 ->
+   combine (upd_Znth i l1 x) l2 = upd_Znth i (combine l1 l2) (x, Znth i l2).
+Proof.
+  intros; rewrite <- combine_upd_Znth by auto.
+  erewrite upd_Znth_triv with (l := l2); eauto; omega.
+Qed.
+
+Corollary combine_upd_Znth2 : forall {A B}{d: Inhabitant A} (l1 : list A) (l2 : list B) i x, 0 <= i < Zlength l1 ->
+  Zlength l1 = Zlength l2 -> combine l1 (upd_Znth i l2 x) = upd_Znth i (combine l1 l2) (Znth i l1, x).
+Proof.
+  intros; rewrite <- combine_upd_Znth by auto.
+  erewrite upd_Znth_triv with (l := l1); eauto; omega.
+Qed.
+
+Lemma in_concat : forall {A} (l : list (list A)) x, In x (concat l) <-> exists l1, In x l1 /\ In l1 l.
+Proof.
+  induction l; simpl; intros.
+  - split; [|intros (? & ? & ?)]; contradiction.
+  - rewrite in_app, IHl; split.
+    + intros [? | (? & ? & ?)]; eauto.
+    + intros (? & ? & [? | ?]); subst; eauto.
+Qed.
+
+Lemma length_concat : forall {A} (l : list (list A)), length (concat l) = fold_right plus O (map (@length A) l).
+Proof.
+  induction l; auto; simpl.
+  rewrite app_length, IHl; auto.
+Qed.
+
+Lemma length_concat_min : forall {A}{d: Inhabitant A} (l : list (list A)) i (Hi : 0 <= i < Zlength l),
+  (length (Znth i l) <= length (concat l))%nat.
+Proof.
+  induction l; simpl; intros; [rewrite Zlength_nil in *; omega|].
+  rewrite app_length; destruct (Z.eq_dec i 0).
+  - subst; rewrite Znth_0_cons; omega.
+  - rewrite Znth_pos_cons by omega.
+    rewrite Zlength_cons in *; etransitivity; [apply IHl|]; omega.
+Qed.
+
+Lemma length_concat_upd : forall {A} {d: Inhabitant A} l i (l' : list A) (Hi : 0 <= i < Zlength l),
+  length (concat (upd_Znth i l l')) = (length (concat l) + length l' - length (Znth i l))%nat.
+Proof.
+  induction l; intros; [rewrite Zlength_nil in *; omega|].
+  destruct (Z.eq_dec i 0).
+  - subst; rewrite upd_Znth0, Znth_0_cons, sublist_1_cons.
+    rewrite Zlength_cons in *; rewrite sublist_same by (auto; omega); simpl.
+    rewrite !app_length; omega.
+  - rewrite upd_Znth_cons, Znth_pos_cons by omega; simpl.
+    rewrite Zlength_cons in *.
+    rewrite !app_length, IHl by omega.
+    exploit (length_concat_min l (i - 1)); omega.
+Qed.
+
+Lemma incl_nil : forall {A} (l : list A), incl [] l.
+Proof.
+  repeat intro; contradiction.
+Qed.
+Hint Resolve incl_nil : list.
+
+Lemma incl_cons_out : forall {A} (a : A) l1 l2, incl l1 (a :: l2) -> ~In a l1 -> incl l1 l2.
+Proof.
+  intros; intros ? Hin; specialize (H _ Hin); destruct H; auto; subst; contradiction.
+Qed.
+
+Lemma In_upd_Znth : forall {A} i l (x y : A), In x (upd_Znth i l y) -> x = y \/ In x l.
+Proof.
+  unfold upd_Znth; intros.
+  rewrite in_app in H; destruct H as [? | [? | ?]]; auto; right; eapply sublist_In; eauto.
+Qed.
+
+Lemma upd_Znth_In : forall {A} i l (x : A), In x (upd_Znth i l x).
+Proof.
+  intros; unfold upd_Znth.
+  rewrite in_app; simpl; auto.
+Qed.
+
+Lemma Znth_cons_eq : forall {A}{d : Inhabitant A} i x l, 
+   Znth i (x :: l) = if Z.eq_dec i 0 then x else Znth (i - 1) l.
+Proof.
+  intros.
+  destruct (Z.eq_dec i 0); [subst; apply Znth_0_cons|].
+  destruct (zlt i 0); [rewrite !Znth_underflow; auto; omega|].
+  apply Znth_pos_cons; omega.
+Qed.
+
+Lemma NoDup_Znth_inj : forall {A} {d : Inhabitant A} l i j (HNoDup : NoDup l)
+  (Hi : 0 <= i < Zlength l) (Hj : 0 <= j < Zlength l) (Heq : Znth i l = Znth j l ),
+  i = j.
+Proof.
+  induction l; intros.
+  { rewrite Zlength_nil in *; omega. }
+  inv HNoDup.
+  rewrite Zlength_cons in *.
+  rewrite !Znth_cons_eq in Heq.
+  destruct (Z.eq_dec i 0), (Z.eq_dec j 0); subst; auto.
+  - contradiction H1; apply Znth_In; omega.
+  - contradiction H1; apply Znth_In; omega.
+  - exploit (IHl (i - 1) (j - 1)); auto; omega.
+Qed.
+
+Lemma NoDup_Znth_iff : forall {A}{d: Inhabitant A} (l : list A),
+  NoDup l <-> forall i j (Hi : 0 <= i < Zlength l)
+                            (Hj : 0 <= j < Zlength l), Znth i l = Znth j l -> i = j.
+Proof.
+  split; intros; [eapply NoDup_Znth_inj; eauto|].
+  induction l; rewrite ?Zlength_cons in *; constructor.
+  - intro Hin; eapply In_Znth in Hin; destruct Hin as (j & ? & Hj).
+    exploit (H 0 (j + 1)); try omega.
+    rewrite !Znth_cons_eq; simpl.
+    if_tac; [omega|].
+    rewrite Z.add_simpl_r; eauto.
+  - apply IHl; intros.
+    exploit (H (i + 1) (j + 1)); try omega.
+    rewrite !Znth_cons_eq, !Z.add_simpl_r.
+    if_tac; [omega|].
+    if_tac; [omega | auto].
+Qed.
+
+Lemma concat_less_incl : forall {A} l i (l1 l2 : list A) (Hi : 0 <= i < Zlength l)
+  (Hless : Znth i l = l1 ++ l2), incl (concat (upd_Znth i l l1)) (concat l).
+Proof.
+  intros.
+  intros ? Hin.
+  rewrite in_concat in Hin; rewrite in_concat.
+  destruct Hin as (? & ? & Hin).
+  apply In_upd_Znth in Hin; destruct Hin; eauto; subst.
+  do 2 eexists; [rewrite in_app; left; eauto|].
+  rewrite <- Hless; apply Znth_In; auto.
+Qed.
+
+Lemma NoDup_app : forall {A} (l1 l2 : list A), NoDup (l1 ++ l2) ->
+  NoDup l1 /\ NoDup l2 /\ forall x, In x l1 -> ~In x l2.
+Proof.
+  induction l1; intros.
+  - repeat split; auto; constructor.
+  - inv H.
+    exploit IHl1; eauto; intros (? & ? & ?).
+    rewrite in_app in *.
+    repeat split; auto.
+    + constructor; auto.
+    + intros ? [? | ?]; auto; subst; auto.
+Qed.
+
+Lemma NoDup_app_iff : forall {A} (l1 l2 : list A), NoDup (l1 ++ l2) <->
+  NoDup l1 /\ NoDup l2 /\ forall x, In x l1 -> ~In x l2.
+Proof.
+  intros; split; [apply NoDup_app|].
+  intros (? & ? & Hsep); induction l1; auto.
+  inv H; simpl; constructor.
+  - rewrite in_app_iff; intros [? | ?]; [contradiction|].
+    eapply Hsep; simpl; eauto.
+  - apply IHl1; auto.
+    intros; apply Hsep; simpl; auto.
+Qed.
+
+Corollary NoDup_app_swap : forall {A} (l1 l2 : list A), NoDup (l1 ++ l2) <-> NoDup (l2 ++ l1).
+Proof.
+  intros; rewrite !NoDup_app_iff; split; intros (? & ? & Hsep); repeat split; auto; repeat intro; eapply Hsep;
+    eauto.
+Qed.
+
+Lemma NoDup_concat_less : forall {A} l i (l1 l2 : list A) (Hl : NoDup (concat l))
+  (Hi : 0 <= i < Zlength l) (Hless : Znth i l = l1 ++ l2),
+  NoDup (concat (upd_Znth i l l1)).
+Proof.
+  induction l; simpl; intros; [rewrite Zlength_nil in *; omega|].
+  rewrite Zlength_cons in *.
+  destruct (Z.eq_dec i 0).
+  - subst; rewrite upd_Znth0, Zlength_cons, sublist_1_cons, sublist_same by (auto; omega); simpl.
+    rewrite Znth_0_cons in Hless; subst.
+    rewrite <- app_assoc, NoDup_app_swap, <- app_assoc, NoDup_app_iff, NoDup_app_swap in Hl; tauto.
+  - rewrite upd_Znth_cons by omega; simpl.
+    rewrite Znth_pos_cons in Hless by omega.
+    rewrite NoDup_app_iff in Hl; rewrite NoDup_app_iff.
+    destruct Hl as (? & ? & Hsep).
+    split; [auto|]; split.
+    + eapply IHl; eauto; omega.
+    + intros ?? Hin; eapply Hsep; eauto.
+      eapply concat_less_incl; eauto; omega.
+Qed.
+
+Lemma Forall2_Znth : forall {A B}{d1: Inhabitant A}{d2: Inhabitant B} (P : A -> B -> Prop) l1 l2 (Hall : Forall2 P l1 l2) i
+  (Hi : 0 <= i < Zlength l1), P (Znth i l1) (Znth i l2).
+Proof.
+  induction 1; intros.
+  { rewrite Zlength_nil in *; omega. }
+  rewrite Zlength_cons in *.
+  destruct (Z.eq_dec i 0).
+  - subst; rewrite !Znth_0_cons; auto.
+  - rewrite !Znth_pos_cons; try omega.
+    apply IHHall; omega.
+Qed.
+
+Lemma Forall2_app_inv : forall {A B} (P : A -> B -> Prop) l1 l2 l3 l4 (Hlen : length l1 = length l3),
+  Forall2 P (l1 ++ l2) (l3 ++ l4) -> Forall2 P l1 l3 /\ Forall2 P l2 l4.
+Proof.
+  induction l1; destruct l3; try discriminate; auto; intros.
+  inv H; inv Hlen.
+  exploit IHl1; eauto; intros (? & ?); split; [constructor|]; auto.
+Qed.
+
+Lemma Forall2_firstn : forall {A B} (P : A -> B -> Prop) l1 l2 n, Forall2 P l1 l2 ->
+  Forall2 P (firstn n l1) (firstn n l2).
+Proof.
+  intros; revert n; induction H; intro.
+  - rewrite !firstn_nil; auto.
+  - destruct n; simpl; auto.
+Qed.
+
+Lemma Forall2_length {A B} {f:A -> B -> Prop} {l1 l2} (F:Forall2 f l1 l2): length l1 = length l2.
+Proof. induction F; trivial. simpl; rewrite IHF. trivial. Qed.
+
+Lemma Forall2_Zlength {A B} {f:A -> B -> Prop} {l1 l2} (F:Forall2 f l1 l2): Zlength l1 = Zlength l2.
+Proof. do 2 rewrite Zlength_correct. rewrite (Forall2_length F). trivial. Qed.
+
+Lemma Forall2_upd_Znth : forall {A B} (P : A -> B -> Prop) l1 l2 i x1 x2, Forall2 P l1 l2 ->
+  P x1 x2 -> 0 <= i <= Zlength l1 -> Forall2 P (upd_Znth i l1 x1) (upd_Znth i l2 x2).
+Proof.
+  intros; unfold upd_Znth.
+  pose proof (Forall2_Zlength H) as Hlen.
+  erewrite <- sublist_same with (al := l1), sublist_split with (mid := i) in H; auto; try omega.
+  erewrite <- sublist_same with (al := l2), sublist_split with (al := l2)(mid := i) in H; auto; try omega.
+  apply Forall2_app_inv in H.
+  destruct H as (? & Hall); apply Forall2_app; auto.
+  constructor; auto.
+  destruct (Z.eq_dec i (Zlength l1)).
+  - rewrite !sublist_nil_gen; auto; omega.
+  - rewrite Z.add_comm.
+    replace (Zlength l1) with (Zlength l1 - i + i) by omega.
+    replace (Zlength l2) with (Zlength l2 - i + i) by omega.
+    erewrite <- !sublist_sublist with (j := Zlength l1); try omega.
+    inversion Hall as [Hl1 Hl2 | ?????? Hl1 Hl2].
+    + rewrite !Hlen, <- Hl2.
+      unfold sublist; rewrite !skipn_nil, !firstn_nil; auto.
+    + rewrite sublist_1_cons, !Hlen, <- Hl2, sublist_1_cons.
+      unfold sublist; simpl; apply Forall2_firstn; auto.
+  - apply Nat2Z.inj; rewrite <- !Zlength_correct.
+    autorewrite with sublist; auto.
+Qed.
+
+Lemma Forall2_impl' : forall {A B} (P Q : A -> B -> Prop) l1 l2,
+  (forall a b, In a l1 -> In b l2 -> P a b -> Q a b) -> Forall2 P l1 l2 -> Forall2 Q l1 l2.
+Proof.
+  induction 2; simpl in *; auto.
+Qed.
+
+Lemma Forall2_impl : forall {A B} (P Q : A -> B -> Prop), (forall a b, P a b -> Q a b) ->
+  forall l1 l2, Forall2 P l1 l2 -> Forall2 Q l1 l2.
+Proof.
+  induction 2; auto.
+Qed.
+
+Lemma map_id_eq : forall {A} (l : list A), map (@id A) l = l.
+Proof.
+  induction l; auto.
+  simpl; apply f_equal; auto.
+Qed.
+
+Lemma Forall2_map : forall {A B C D} (P : A -> B -> Prop) (f1 : C -> A) (f2 : D -> B) l1 l2,
+  Forall2 P (map f1 l1) (map f2 l2) <-> Forall2 (fun a b => P (f1 a) (f2 b)) l1 l2.
+Proof.
+  induction l1.
+  - split; intro H.
+    + destruct l2; auto; inv H.
+    + inv H; simpl; auto.
+  - split; intro H.
+    + destruct l2; inv H.
+      rewrite IHl1 in *; constructor; auto.
+    + inv H; simpl; constructor; auto.
+      rewrite IHl1; auto.
+Qed.
+
+Corollary Forall2_map1 : forall {A B C} (P : A -> B -> Prop) (f : C -> A) l1 l2, Forall2 P (map f l1) l2 <->
+  Forall2 (fun a b => P (f a) b) l1 l2.
+Proof.
+  intros; rewrite <- (map_id_eq l2) at 1; apply Forall2_map.
+Qed.
+
+Corollary Forall2_map2 : forall {A B C} (P : A -> B -> Prop) (f : C -> B) l1 l2, Forall2 P l1 (map f l2) <->
+  Forall2 (fun a b => P a (f b)) l1 l2.
+Proof.
+  intros; rewrite <- (map_id_eq l1) at 1; apply Forall2_map.
+Qed.
+
+Lemma sublist_max_length : forall {A} i j (al : list A), Zlength (sublist i j al) <= Zlength al.
+Proof.
+  intros; unfold sublist.
+  rewrite Zlength_firstn, Zlength_skipn.
+  rewrite Z.min_le_iff; right.
+  pose proof (Zlength_nonneg al).
+  apply Z.max_lub; try omega.
+  rewrite <- Z.le_sub_nonneg; apply Z.le_max_l.
+Qed.
+
+Lemma sublist_of_nil : forall {A} i j, sublist i j (@nil A) = [].
+Proof.
+  intros; unfold sublist.
+  rewrite skipn_nil, firstn_nil; auto.
+Qed.
+
+Lemma sublist_0_cons : forall {A} j x (l : list A), j > 0 ->
+  sublist 0 j (x :: l) = x :: sublist 0 (j - 1) l.
+Proof.
+  intros; unfold sublist; simpl.
+  destruct (Z.to_nat (j - 0)) eqn: Hminus.
+  - apply Z.gt_lt in H; rewrite Z2Nat.inj_lt in H; try omega.
+    rewrite Z2Nat.inj_sub in Hminus; omega.
+  - simpl; repeat f_equal.
+    rewrite Z.sub_0_r in *.
+    rewrite Z2Nat.inj_sub, Hminus; simpl; omega.
+Qed.
+
+Lemma sublist_S_cons : forall {A} i j x (l : list A), i > 0 ->
+  sublist i j (x :: l) = sublist (i - 1) (j - 1) l.
+Proof.
+  intros; unfold sublist; simpl.
+  destruct (Z.to_nat i) eqn: Hi.
+  - apply Z.gt_lt in H; rewrite Z2Nat.inj_lt in H; omega.
+  - simpl.
+    f_equal; f_equal; try omega.
+    rewrite Z2Nat.inj_sub, Hi; simpl; omega.
+Qed.
+
+Lemma Forall2_sublist : forall {A B} (P : A -> B -> Prop) l1 l2 i j, Forall2 P l1 l2 -> 0 <= i ->
+  Forall2 P (sublist i j l1) (sublist i j l2).
+Proof.
+  intros; revert j; revert dependent i; induction H; intros.
+  - rewrite !sublist_of_nil; constructor.
+  - destruct (Z_le_dec j i); [rewrite !sublist_nil_gen; auto; constructor|].
+    destruct (Z.eq_dec i 0).
+    + subst; rewrite !sublist_0_cons by omega.
+      constructor; auto.
+    + rewrite !sublist_S_cons by omega.
+      apply IHForall2; omega.
+Qed.
+
+Lemma Forall_last : forall {A} (P : A -> Prop) d l, Forall P l -> P d -> P (last l d).
+Proof.
+  destruct l; auto.
+  exploit (@app_removelast_last _ (a :: l) d); [discriminate | intro Hlast].
+  intros; rewrite Forall_forall in H; apply H.
+  rewrite Hlast at 2; rewrite in_app; simpl; auto.
+Qed.
+
+Lemma last_map : forall {A B} (f : A -> B) d l, f (last l d) = last (map f l) (f d).
+Proof.
+  induction l; auto; simpl.
+  destruct l; auto.
+Qed.
+
+Lemma In_removelast : forall {A} (l : list A) x, In x (removelast l) -> In x l.
+Proof.
+  induction l; auto; simpl; intros.
+  destruct l; auto.
+  destruct H; auto.
+Qed.
+
+Definition nil_dec {A} (l : list A) : {l = []} + {l <> []}.
+Proof.
+  destruct l; auto.
+  right; discriminate.
+Qed.
+
+Lemma Forall2_upd_Znth_l : forall {A B}{d: Inhabitant B} (P : A -> B -> Prop) l1 l2 i x, Forall2 P l1 l2 ->
+  P x (Znth i l2) -> 0 <= i < Zlength l1 -> Forall2 P (upd_Znth i l1 x) l2.
+Proof.
+  intros.
+  erewrite <- upd_Znth_triv with (l := l2)(i0 := i); eauto.
+  apply Forall2_upd_Znth; eauto; omega.
+  apply Forall2_Zlength in H; omega.
+Qed.
+
+Lemma Forall2_upd_Znth_r : forall {A B}{d: Inhabitant A} (P : A -> B -> Prop) l1 l2 i x, Forall2 P l1 l2 ->
+  P (Znth i l1) x -> 0 <= i < Zlength l1 -> Forall2 P l1 (upd_Znth i l2 x).
+Proof.
+  intros.
+  erewrite <- upd_Znth_triv with (l := l1)(i0 := i) by (eauto; omega).
+  apply Forall2_upd_Znth; eauto.
+  apply Forall2_Zlength in H; omega.
+Qed.
+
+Lemma Znth_inbounds : forall {A}{d: Inhabitant A} i (l : list A), 
+    Znth i l <> default -> 0 <= i < Zlength l.
+Proof.
+  intros.
+  destruct (zlt i 0); [contradiction H; apply Znth_underflow; auto|].
+  destruct (Z_lt_dec i (Zlength l)); [omega|].
+  rewrite Znth_overflow in H; [contradiction H; auto | omega].
+Qed.
+
+Lemma upd_Znth_diff' : forall {A}{d: Inhabitant A} i j l (u : A),
+    0 <= j < Zlength l -> i <> j ->
+  Znth i (upd_Znth j l u) = Znth i l.
+Proof.
+  intros.
+  destruct (zlt i 0).
+  { rewrite !Znth_underflow; auto. }
+  destruct (zlt i (Zlength l)).
+  apply upd_Znth_diff; auto; omega.
+  { rewrite !Znth_overflow; auto.
+    rewrite upd_Znth_Zlength; auto. }
+Qed.
+
+Lemma list_nth_error_eq : forall {A} (l1 l2 : list A)
+  (Heq : forall j, nth_error l1 j = nth_error l2 j), l1 = l2.
+Proof.
+  induction l1; destruct l2; auto; intros; try (specialize (Heq O); simpl in Heq; discriminate).
+  erewrite IHl1.
+  - specialize (Heq O); inv Heq; eauto.
+  - intro j; specialize (Heq (S j)); auto.
+Qed.
+
+Lemma upd_Znth_twice : forall {A} i l (x y : A), 0 <= i < Zlength l ->
+  upd_Znth i (upd_Znth i l x) y = upd_Znth i l y.
+Proof.
+  intros; unfold upd_Znth.
+  rewrite !sublist_app; rewrite ?Zlength_app, ?Zlength_cons, ?Zlength_sublist; try omega.
+  rewrite 2Z.min_l, 2Z.min_r, 2Z.max_r, 2Z.max_l; try omega.
+  rewrite !sublist_nil, app_nil_r; simpl.
+  rewrite sublist_S_cons, !sublist_sublist; try omega.
+  f_equal; f_equal; [|f_equal]; omega.
+Qed.
+
+Lemma hd_Znth : forall {A}{d: Inhabitant A} (l : list A), hd default l = Znth 0 l.
+Proof.
+  destruct l; auto.
+Qed.
+
+Fixpoint upto n :=
+  match n with
+  | O => []
+  | S n' => 0 :: map Z.succ (upto n')
+  end.
+
+Opaque Z.of_nat.
+
+Lemma upto_app : forall n m, upto (n + m) = upto n ++ map (fun i => Z.of_nat n + i) (upto m).
+Proof.
+  induction n; simpl; intro.
+  - rewrite map_id; auto.
+  - rewrite IHn, map_app, map_map, Nat2Z.inj_succ; f_equal; f_equal.
+    apply map_ext; intro; omega.
+Qed.
+
+Lemma upto_length : forall n, length (upto n) = n.
+Proof.
+  induction n; auto; simpl.
+  rewrite map_length, IHn; auto.
+Qed.
+
+Corollary Zlength_upto : forall n, Zlength (upto n) = Z.of_nat n.
+Proof.
+  intro; rewrite Zlength_correct, upto_length; auto.
+Qed.
+
+Lemma skipn_cons : forall {A}{d: Inhabitant A} n (l : list A), (length l > n)%nat ->
+  skipn n l = Znth (Z.of_nat n) l :: skipn (S n) l.
+Proof.
+  induction n; intros; simpl; destruct l; simpl in *; try omega; auto.
+  { inversion H. }
+  rewrite Nat2Z.inj_succ.
+  rewrite Znth_pos_cons; [|omega].
+  unfold Z.succ; rewrite Z.add_simpl_r.
+  erewrite IHn; auto; omega.
+Qed.
+
+Lemma Znth_nil : forall `{Inhabitant} n, Znth n [] = default.
+Proof.
+  intros; unfold Znth.
+  if_tac; auto.
+  destruct (Z.to_nat n); auto.
+Qed.
+
+Lemma Znth_upto : forall d m n, 
+  0 <= n < Z.of_nat m -> @Znth _ d n (upto m) = n.
+Proof.
+  induction m; simpl; intros.
+  - rewrite Znth_nil; simpl in *; rewrite Nat2Z.inj_0 in *; omega.
+  - destruct (Z.eq_dec n 0).
+    + subst; apply Znth_0_cons.
+    + rewrite Nat2Z.inj_succ in *.
+      rewrite Znth_pos_cons by omega.
+      rewrite Znth_map. rewrite IHm. omega. omega.
+      rewrite Zlength_upto. omega.
+Qed.
+
+Lemma sublist_upto : forall n a b, 0 <= a <= b -> sublist a b (upto n) = map (Z.add a) (upto (Min.min n (Z.to_nat b) - Z.to_nat a)).
+Proof.
+  induction n; intros.
+  - simpl; rewrite sublist_of_nil by omega; auto.
+  - simpl.
+    destruct (Z.to_nat b) eqn: Hb.
+    { apply f_equal with (f := Z.of_nat) in Hb; rewrite Z2Nat.id in Hb by omega; subst.
+      change (Z.of_nat O) with 0 in H.
+      assert (a = 0) by omega; subst.
+      rewrite sublist_nil; auto. }
+    destruct (zlt 0 b).
+    destruct (Z.eq_dec a 0).
+    + subst; rewrite sublist_0_cons, sublist_map, IHn by omega; simpl; f_equal.
+      rewrite Z2Nat.inj_sub, Hb by omega; simpl.
+      rewrite !Nat.sub_0_r, !map_map; auto.
+    + rewrite sublist_S_cons, sublist_map, IHn by omega; simpl.
+      destruct (Z.to_nat a) eqn: Ha.
+      { apply f_equal with (f := Z.of_nat) in Ha; rewrite Z2Nat.id in Ha by omega; contradiction. }
+      rewrite !Z2Nat.inj_sub, Ha, Hb by omega; simpl.
+      rewrite !Nat.sub_0_r, !map_map; apply map_ext; intros; omega.
+    + destruct (Z.eq_dec b 0); try omega.
+      subst; discriminate.
+Qed.
+
+Transparent Z.of_nat.
+
+Lemma In_upto : forall n i, In i (upto n) <-> 0 <= i < Z.of_nat n.
+Proof.
+  induction n; intro.
+  - simpl; split; try contradiction; omega.
+  - rewrite Nat2Z.inj_succ; simpl.
+    rewrite in_map_iff; split.
+    + intros [? | ?]; [omega|].
+      destruct H as (? & ? & ?); subst; rewrite IHn in *; omega.
+    + intro; destruct (Z.eq_dec i 0); [auto | right].
+      exists (i - 1); rewrite IHn; omega.
+Qed.
+
+Lemma Forall2_eq_upto : forall {A B}{d1: Inhabitant A}{d2: Inhabitant B} (P : A -> B -> Prop) l1 l2, Forall2 P l1 l2 <->
+  Zlength l1 = Zlength l2 /\ Forall (fun i => P (Znth i l1) (Znth i l2)) (upto (Z.to_nat (Zlength l1))).
+Proof.
+  induction l1; destruct l2; rewrite ?Zlength_cons, ?Zlength_nil; try solve [split; intro H; inv H;
+    try (rewrite Zlength_correct in *; omega)]; simpl.
+  - change (upto 0) with (@nil Z); split; auto.
+  - rewrite Z2Nat.inj_succ by (apply Zlength_nonneg).
+    rewrite <- Nat.add_1_l, upto_app, Forall_app, Forall_map.
+    change (upto 1) with [0]; split; intro H.
+    + inversion H as [|????? Hall]; subst.
+      rewrite IHl1 in Hall; destruct Hall as (? & Hall).
+      split; [congruence|].
+      split; auto.
+      rewrite Forall_forall in *; intros ? Hin.
+      unfold Basics.compose.
+      specialize (Hall _ Hin).
+      rewrite In_upto in Hin.
+      rewrite !Znth_pos_cons, Z.add_simpl_l by (simpl Z.of_nat; omega); auto.
+    + destruct H as (? & Ha & Hall); inversion Ha as [|?? HP]; subst.
+      rewrite !Znth_0_cons in HP.
+      constructor; auto.
+      rewrite IHl1; split; [omega|].
+      rewrite Forall_forall in *; intros ? Hin.
+      specialize (Hall _ Hin).
+      rewrite In_upto in Hin; unfold Basics.compose in Hall.
+      rewrite !Znth_pos_cons, Z.add_simpl_l in Hall by (simpl Z.of_nat; omega); auto.
+Qed.
+
+Lemma Forall2_forall_Znth : forall {A B}{d1: Inhabitant A}{d2: Inhabitant B}  (P : A -> B -> Prop) l1 l2,
+  Forall2 P l1 l2 <->
+  Zlength l1 = Zlength l2 /\ (forall i, 0 <= i < Zlength l1 -> P (Znth i l1) (Znth i l2)).
+Proof.
+  intros; rewrite Forall2_eq_upto, Forall_forall.
+  setoid_rewrite In_upto.
+  rewrite Z2Nat.id by (apply Zlength_nonneg).
+  reflexivity.
+Qed.
