progs/invariants.v
@@ -1,5 +1,4 @@
-From stdpp Require Export coPset.
-Require Import VST.msl.ghost.
+Require Export VST.veric.invariants.
 Require Import VST.msl.ghost_seplog.
 Require Import VST.msl.sepalg_generators.
 Require Import VST.veric.compcert_rmaps.
@@ -18,9 +17,7 @@ Qed.
 
 Lemma cored_dup_cored : forall P, P && cored |-- ((P && cored) * (P && cored)) && cored.
 Proof.
-  intros; apply andp_right.
-  - apply cored_dup.
-  - apply andp_left2; auto.
+  exact cored_dup_cored.
 Qed.
 
 Lemma cored_duplicable : cored = cored * cored.
@@ -35,21 +32,13 @@ Qed.
 
 Lemma cored_sepcon: forall P Q, (P && cored) * (Q && cored) |-- (P * Q) && cored.
 Proof.
-  intros.
-  apply andp_right.
-  + apply sepcon_derives; apply andp_left1; auto.
-  + eapply derives_trans; [apply sepcon_derives; apply andp_left2, derives_refl|].
-      rewrite <- cored_duplicable; auto.
+  exact cored_sepcon.
 Qed.
 
 Lemma cored_dup_gen : forall P, P |-- cored -> P |-- P * P.
 Proof.
-  intros.
-  erewrite (add_andp P) by apply H; apply cored_dup.
+  exact cored_dup_gen.
 Qed.
-
-Require Import VST.veric.bi.
-Require Import VST.msl.sepalg.
 
 Lemma cored_emp: (cored |-- |==> emp)%I.
 Proof.
@@ -61,716 +50,39 @@ Proof.
   apply own.emp_cored.
 Qed.
 
-Section Invariants.
-
-Program Instance unit_PCM : Ghost := { valid a := True; Join_G a b c := True }.
-
-Definition pred_of (P : mpred) := SomeP rmaps.Mpred (fun _ => P).
-
-Definition agree g (P : mpred) := own(RA := unit_PCM) g tt (pred_of P).
-
-Lemma agree_dup : forall g P, agree g P = agree g P * agree g P.
+Lemma iter_sepcon_eq : forall A, @invariants.iter_sepcon A = @iter_sepcon mpred A _ _.
 Proof.
-  intros; apply own_op; constructor.
-Qed.
-
-Lemma agree_join : forall g P1 P2, agree g P1 * agree g P2 |-- (|> P1 -* |> P2) * agree g P1.
-Proof.
-  intros.
-  change (predicates_hered.derives (agree g P1 * agree g P2) ((|> P1 -* |> P2) * agree g P1)).
-  intros ? (? & ? & ? & H1 & H2).
-  do 3 eexists; [apply core_unit|].
-  pose proof (ghost_of_join _ _ _ H) as J.
-  change (agree g P1) with (own.own(RA := unit_PCM) g tt (pred_of P1)) in H1.
-  destruct H1 as (? & Hid & H1).
-  change (agree g P2) with (own.own(RA := unit_PCM) g tt (pred_of P2)) in H2.
-  destruct H2 as (? & ? & H2).
-  erewrite H1, H2, !own.ghost_fmap_singleton in J.
-  apply own.singleton_join_inv in J as ([] & J & Jg).
-  inv J; simpl in *.
-  inv H4.
-  apply SomeP_inj in H5.
-  destruct (join_level _ _ _ H) as [Hl1 Hl2]; erewrite Hl1, Hl2 in *.
-  assert (approx (level a) P1 = approx (level a) P2) as Heq.
-  { apply (@equal_f _ _ (fun _ : list Type => approx (level a) P1) (fun _ : list Type => approx (level a) P2));
-      auto.
-    apply nil. }
-  split.
-  - intros ??? Hl J HP1 ? Ha'.
-    pose proof (level_core a).
-    pose proof (necR_level _ _ Hl).
-    apply nec_identity in Hl; [|apply core_identity].
-    destruct (join_level _ _ _ J).
-    apply Hl in J; subst.
-    specialize (HP1 _ Ha').
-    apply laterR_level in Ha'.
-    assert ((approx (level a) P1) a') as HP1'.
-    { split; auto; lia. }
-    rewrite Heq in HP1'; destruct HP1'; auto.
-  - exists I; split.
-    + intro l; simpl.
-      apply (resource_at_join _ _ _ l) in H.
-      apply Hid in H as <-; auto.
-    + simpl; erewrite Jg, own.ghost_fmap_singleton; simpl.
-      repeat f_equal; auto.
-      inv H3; f_equal.
-      destruct c0; apply exist_ext; auto.
-Qed.
-
-Lemma agree_join2 : forall g P1 P2, agree g P1 * agree g P2 |-- (|> P1 -* |> P2) * agree g P2.
-Proof.
-  intros.
-  change (predicates_hered.derives (agree g P1 * agree g P2) ((|> P1 -* |> P2) * agree g P2)).
-  intros ? (? & ? & ? & H1 & H2).
-  do 3 eexists; [apply core_unit|].
-  pose proof (ghost_of_join _ _ _ H) as J.
-  change (agree g P1) with (own.own(RA := unit_PCM) g tt (pred_of P1)) in H1.
-  destruct H1 as (? & Hid & H1).
-  change (agree g P2) with (own.own(RA := unit_PCM) g tt (pred_of P2)) in H2.
-  destruct H2 as (? & ? & H2).
-  erewrite H1, H2, !own.ghost_fmap_singleton in J.
-  apply own.singleton_join_inv in J as ([] & J & Jg).
-  inv J; simpl in *.
-  inv H4.
-  apply SomeP_inj in H5.
-  destruct (join_level _ _ _ H) as [Hl1 Hl2]; erewrite Hl1, Hl2 in *.
-  assert (approx (level a) P1 = approx (level a) P2) as Heq.
-  { apply (@equal_f _ _ (fun _ : list Type => approx (level a) P1) (fun _ : list Type => approx (level a) P2));
-      auto.
-    apply nil. }
-  split.
-  - intros ??? Hl J HP1 ? Ha'.
-    pose proof (level_core a).
-    pose proof (necR_level _ _ Hl).
-    apply nec_identity in Hl; [|apply core_identity].
-    destruct (join_level _ _ _ J).
-    apply Hl in J; subst.
-    specialize (HP1 _ Ha').
-    apply laterR_level in Ha'.
-    assert ((approx (level a) P1) a') as HP1'.
-    { split; auto; lia. }
-    rewrite Heq in HP1'; destruct HP1'; auto.
-  - exists I; split.
-    + intro l; simpl.
-      apply (resource_at_join _ _ _ l) in H.
-      apply Hid in H as <-; auto.
-    + simpl; erewrite Jg, own.ghost_fmap_singleton; simpl.
-      repeat f_equal; auto.
-      inv H3; f_equal.
-      destruct c0; apply exist_ext; auto.
-Qed.
-
-Inductive list_join {P : Ghost} : Join (list (option G)) :=
-  | list_join_nil_l m: list_join nil m m
-  | list_join_nil_r m: list_join m nil m
-  | list_join_cons a1 a2 m1 m2 a3 m3: join a1 a2 a3 -> list_join m1 m2 m3 ->
-      list_join (a1 :: m1) (a2 :: m2) (a3 :: m3).
-Existing Instance list_join.
-
-Lemma list_join_inv: forall {P : Ghost} (l1 l2 l3 : list (option G)), list_join l1 l2 l3 ->
-match l1, l2 with
-| nil, _ => l3 = l2
-| _, nil => l3 = l1
-| a1 :: l1, a2 :: l2 => match l3 with nil => False
-                        | a3 :: l3 => join a1 a2 a3 /\ list_join l1 l2 l3 end
-end.
-Proof.
-  induction 1; simpl; auto.
-  destruct m; simpl; auto.
-Qed.
-
-Program Instance list_PCM (P : Ghost) : Ghost := { valid a := True; Join_G := list_join(*; core2 := map core2*) }.
-Next Obligation.
-Proof.
-  exists (fun _ => nil); auto; constructor.
-Defined.
-Next Obligation.
-  constructor.
-    + intros until 1.
-      revert z'; induction H; inversion 1; auto; subst.
-      f_equal; eauto.
-      eapply join_eq; eauto.
-    + induction a; intros ???? J1 J2; eapply list_join_inv in J1; subst.
-      { exists e; split; auto; constructor. }
-      destruct b; subst; [eexists; split; eauto; constructor|].
-      destruct d; [contradiction|].
-      destruct J1 as [Jc1 J1].
-      apply list_join_inv in J2.
-      destruct c; subst; [eexists; split; eauto; constructor; auto|].
-      destruct e; [contradiction|].
-      destruct J2 as [Jc2 J2].
-      destruct (join_assoc Jc1 Jc2) as (f & ? & ?).
-      destruct (IHa _ _ _ _ J1 J2) as (f' & ? & ?).
-      exists (f :: f'); split; constructor; auto.
-    + induction 1; constructor; auto.
-    + intros until 1.
-      revert b'; induction H; inversion 1; auto; subst.
-      f_equal; eauto.
-      eapply join_positivity; eauto.
-Qed.
-
-Definition ghost_list {P : Ghost} g l := own(RA := list_PCM P) g l NoneP.
-
-Definition list_singleton {A} n (a : A) := repeat None n ++ [Some a].
-
-Definition list_incl {A} (l1 l2 : list (option A)) := (length l1 <= length l2)%nat /\
-  forall n a, nth n l1 None = Some a -> nth n l2 None = Some a.
-
-(* up *)
-Lemma app_nth : forall {A} n l1 l2 (d : A),
-  nth n (l1 ++ l2) d = if lt_dec n (length l1) then nth n l1 d else nth (n - length l1) l2 d.
-Proof.
-  intros.
-  if_tac; [rewrite app_nth1 | rewrite app_nth2]; auto; lia.
-Qed.
-
-(* up *)
-Lemma replace_nth_length : forall {A} n l (a : A),
-  length (replace_nth n l a) = length l.
-Proof.
-  induction n; destruct l; simpl; intros; try lia.
-  erewrite IHn by lia; auto.
-Qed.
-
-(* up *)
-Lemma replace_nth_app : forall {A} n l1 l2 (a : A),
-  replace_nth n (l1 ++ l2) a = if lt_dec n (length l1) then replace_nth n l1 a ++ l2
-  else l1 ++ replace_nth (n - length l1) l2 a.
-Proof.
-  induction n; destruct l1; auto; simpl; intros.
-  rewrite IHn.
-  if_tac; if_tac; auto; lia.
-Qed.
-
-Lemma list_join_app : forall {P : Ghost} l1 l2 m1 m2 n1 n2,
-  length l1 = length m1 -> length l1 = length n1 ->
-  list_join l1 m1 n1 -> list_join l2 m2 n2 ->
-  list_join (l1 ++ l2) (m1 ++ m2) (n1 ++ n2).
-Proof.
-  induction 3.
-  - destruct m; auto; discriminate.
-  - destruct m; auto; discriminate.
-  - simpl in *.
-    intros; constructor; auto.
-Qed.
-
-Lemma list_join_None : forall {P : Ghost} n l, (n <= length l)%nat ->
-  list_join (repeat None n) l l.
-Proof.
-  induction n; [constructor|].
-  destruct l; simpl; [lia|].
-  repeat constructor.
-  apply IHn; lia.
-Qed.
-
-Lemma list_join_over : forall {P : Ghost} l l1 l2 l1', (length l <= length l1)%nat ->
-  list_join l l1 l1' -> list_join l (l1 ++ l2) (l1' ++ l2).
-Proof.
-  induction 2; simpl in *.
-  - constructor.
-  - destruct m; [constructor | simpl in *; lia].
-  - constructor; auto.
-    apply IHlist_join; lia.
-Qed.
-
-Lemma singleton_length : forall {A} n (a : A), length (list_singleton n a) = S n.
-Proof.
-  intros; unfold list_singleton.
-  erewrite app_length, repeat_length; simpl; lia.
-Qed.
-
-Lemma list_join_singleton : forall {P : Ghost} n a c l
-  (Hn : (n < length l)%nat) (Hjoin: join (Some a) (nth n l None) (Some c)),
-  list_join (list_singleton n a) l (replace_nth n l (Some c)).
-Proof.
-  induction l using rev_ind; simpl; intros; try lia.
-  rewrite app_length in Hn; simpl in Hn.
-  destruct (eq_dec n (length l)).
-  - subst.
-    erewrite app_nth2, minus_diag in Hjoin by lia; simpl in Hjoin.
-    erewrite replace_nth_app, if_false, minus_diag by lia; simpl.
-    apply list_join_app; try (rewrite repeat_length; auto).
-    + apply list_join_None; auto.
-    + repeat constructor; auto.
-  - assert (n < length l)%nat by lia.
-    erewrite app_nth1 in Hjoin by auto.
-    erewrite replace_nth_app, if_true by auto.
-    apply list_join_over, IHl; auto.
-    rewrite singleton_length; lia.
-Qed.
-
-(* up *)
-Lemma replace_nth_same : forall {A} n l (d : A), replace_nth n l (nth n l d) = l.
-Proof.
-  induction n; destruct l; auto; simpl; intro.
-  rewrite IHn; auto.
+  intros; extensionality f; extensionality l.
+  induction l; auto; simpl.
+  rewrite IHl; auto.
 Qed.
 
 Lemma nth_replace_nth : forall {A} n l a (d : A), (n < length l)%nat ->
   nth n (replace_nth n l a) d = a.
 Proof.
-  induction n; destruct l; auto; simpl; intros; try lia.
-  apply IHn; lia.
+  induction n; destruct l; auto; simpl; intros; try omega.
+  apply IHn; omega.
 Qed.
 
 Lemma nth_replace_nth' : forall {A} n m l a (d : A), m <> n ->
   nth m (replace_nth n l a) d = nth m l d.
 Proof.
-  induction n; destruct l; auto; destruct m; auto; simpl; intros; try lia.
-  apply IHn; lia.
+  induction n; destruct l; auto; destruct m; auto; simpl; intros; try omega.
+  apply IHn; omega.
 Qed.
 
-Lemma Znth_replace_nth : forall {A} {d : Inhabitant A} n l (a : A), (n < length l)%nat ->
-  Znth (Z.of_nat n) (replace_nth n l a) = a.
-Proof.
-  intros; rewrite <- nth_Znth.
-  apply nth_replace_nth; auto.
-Qed.
-
-Lemma Znth_replace_nth' : forall {A} {d : Inhabitant A} n m l (a : A), m <> Z.of_nat n ->
-  Znth m (replace_nth n l a) = Znth m l.
-Proof.
-  intros.
-  destruct (zlt m 0); [rewrite !Znth_underflow; auto|].
-  rewrite <- (Z2Nat.id m) by lia.
-  rewrite <- !nth_Znth; apply nth_replace_nth'.
-  intro; contradiction H; subst.
-  erewrite Z2Nat.id by lia; auto.
-Qed.
-
-Lemma ghost_list_nth : forall {P : Ghost} g n l (a : G) (Ha : nth n l None = Some a),
-  ghost_list g l = ghost_list g (list_singleton n a) * ghost_list g (replace_nth n l None).
-Proof.
-  intros; apply own_op.
-  rewrite <- (replace_nth_same n l None) at 2.
-  destruct (lt_dec n (length l)); [|erewrite nth_overflow in Ha by lia; discriminate].
-  exploit (list_join_singleton n a a (replace_nth n l None)).
-  { rewrite replace_nth_length; auto. }
-  { erewrite nth_replace_nth by auto; constructor. }
-  erewrite replace_nth_replace_nth, Ha; auto.
-Qed.
-
-Lemma list_join_length : forall {P : Ghost} l1 l2 l3, list_join l1 l2 l3 ->
-  (length l1 <= length l3)%nat.
-Proof.
-  induction 1; auto; simpl; lia.
-Qed.
-
-Lemma list_join_filler : forall {P : Ghost} l1 l2 l3 n, list_join l1 l2 l3 ->
-  (n <= length l3 - length l1)%nat -> list_join (l1 ++ repeat None n) l2 l3.
-Proof.
-  induction 1; simpl; intros.
-  - apply list_join_None; lia.
-  - destruct n; [|lia].
-    rewrite app_nil_r; constructor.
-  - constructor; auto.
-Qed.
-
-Lemma list_join_nth : forall {P : Ghost} l1 l2 l3 n, list_join l1 l2 l3 ->
-  join (nth n l1 None) (nth n l2 None) (nth n l3 None).
-Proof.
-  intros; revert n.
-  induction H; intro.
-  - erewrite nth_overflow by (simpl; lia); constructor.
-  - erewrite (nth_overflow []) by (simpl; lia); constructor.
-  - destruct n; simpl; auto.
-Qed.
-
-Lemma list_join_max : forall {P : Ghost} l1 l2 l3, list_join l1 l2 l3 ->
-  length l3 = Max.max (length l1) (length l2).
-Proof.
-  induction 1; simpl; auto.
-  rewrite Nat.max_l; auto; lia.
-Qed.
-
-Lemma list_join_nth_error : forall {P : Ghost} l1 l2 l3 n, list_join l1 l2 l3 ->
-  join (nth_error l1 n) (nth_error l2 n) (nth_error l3 n).
-Proof.
-  intros; revert n.
-  induction H; intro.
-  - rewrite nth_error_nil; constructor.
-  - rewrite nth_error_nil; constructor.
-  - destruct n; simpl; auto.
-    constructor; auto.
-Qed.
-
-Lemma list_join_alt : forall {P : Ghost} l1 l2 l3,
-  list_join l1 l2 l3 <-> forall n, join (nth_error l1 n) (nth_error l2 n) (nth_error l3 n).
-Proof.
-  split; [intros; apply list_join_nth_error; auto|].
-  revert l2 l3; induction l1; simpl; intros.
-  - assert (l2 = l3); [|subst; constructor].
-    apply list_nth_error_eq; intro.
-    specialize (H j); rewrite nth_error_nil in H; inv H; auto.
-  - destruct l2.
-    + assert (a :: l1 = l3); [|subst; constructor].
-      apply list_nth_error_eq; intro.
-      specialize (H j); rewrite nth_error_nil in H; inv H; auto.
-    + destruct l3.
-      { specialize (H O); inv H. }
-      constructor.
-      * specialize (H O); inv H; auto.
-      * apply IHl1; intro.
-        apply (H (S n)).
-Qed.
-
-Lemma nth_error_replace_nth : forall {A} n l (a : A), (n < length l)%nat ->
-  nth_error (replace_nth n l a) n = Some a.
-Proof.
-  induction n; destruct l; auto; simpl; intros; try lia.
-  apply IHn; lia.
-Qed.
-
-Lemma nth_error_replace_nth' : forall {A} n m l (a : A), m <> n ->
-  nth_error (replace_nth n l a) m = nth_error l m.
-Proof.
-  induction n; destruct l; auto; destruct m; auto; simpl; intros; try lia.
-  apply IHn; lia.
-Qed.
-
-Instance list_order A : @PCM_order (list_PCM (discrete_PCM A)) list_incl.
-Proof.
-  constructor.
-  - constructor.
-    + repeat intro; split; auto.
-    + repeat intro.
-      destruct H, H0; split; auto; lia.
-  - intro a.
-    remember (length a) as n.
-    revert dependent a; induction n; intros.
-    + destruct a; inv Heqn.
-      exists b; split; auto.
-      change [] with (core b); apply core_unit.
-    + assert (a <> []) by (intro; subst; discriminate).
-      erewrite (app_removelast_last None) in H, Heqn by auto.
-      erewrite app_length in Heqn; simpl in Heqn.
-      erewrite Nat.add_1_r in Heqn; inv Heqn.
-      specialize (IHn _ eq_refl).
-      destruct (IHn b c) as (c' & ? & ?); auto.
-      { destruct H as [Hlen H].
-        split.
-        { rewrite app_length in Hlen; simpl in *; lia. }
-        intros ?? Hnth.
-        specialize (H n a0).
-        rewrite app_nth in H.
-        if_tac in H; auto.
-        rewrite nth_overflow in Hnth; [discriminate|].
-        apply not_lt; auto. }
-      pose proof (list_join_length _ _ _ H2).
-      pose proof (list_join_length _ _ _ (join_comm H2)).
-      destruct (eq_dec (length (removelast a)) (length c')).
-      * exists (c' ++ [List.last a None]); split.
-        -- erewrite (app_removelast_last None) at 1 by auto.
-           apply join_comm, list_join_over; try lia.
-           apply join_comm in H2; auto.
-        -- split.
-            { destruct H.
-              erewrite app_length in *; simpl in *; lia. }
-            intros ?? Hnth.
-            rewrite app_nth in Hnth.
-            if_tac in Hnth; [apply H3; auto|].
-            destruct (n - length c')%nat eqn: Hminus; [|destruct n0; discriminate].
-            simpl in Hnth.
-            apply H.
-            erewrite app_nth2 by lia.
-            replace (_ - _)%nat with O by lia; auto.
-       * destruct (List.last a None) eqn: Ha.
-         -- exists (replace_nth (length (removelast a)) c' (Some g)).
-            split.
-            ++ apply list_join_alt; intro.
-               pose proof (list_join_max _ _ _ H2) as Hlen.
-               destruct (Max.max_spec (length (removelast a)) (length b)) as [[? Hmax] | [? Hmax]];
-                 setoid_rewrite Hmax in Hlen; try lia.
-               hnf in H2; erewrite list_join_alt in H2.
-               specialize (H2 n0).
-               erewrite (app_removelast_last None) at 1 by auto.
-               rewrite Ha.
-               destruct (lt_dec n0 (length (removelast a))).
-               ** erewrite nth_error_app1 by auto.
-                  erewrite nth_error_replace_nth' by lia; auto.
-               ** erewrite nth_error_app2 by lia.
-                  destruct (eq_dec n0 (length (removelast a))).
-                  { subst; rewrite minus_diag; simpl.
-                    erewrite nth_error_replace_nth by (simpl in *; lia).
-                    destruct (nth_error b (length (removelast a))) eqn: Hb; setoid_rewrite Hb; constructor.
-                    destruct o; constructor.
-                    destruct H0 as [_ Hc].
-                    erewrite nth_error_nth in Hb by auto.
-                    inv Hb.
-                    apply Hc in H7.
-                    destruct H as [_ Hc'].
-                    specialize (Hc' (length (removelast a))).
-                    erewrite app_nth2, minus_diag in Hc' by auto.
-                    setoid_rewrite Hc' in H7; [|reflexivity].
-                    inv H7; constructor; auto. }
-                  { destruct (_ - _)%nat eqn: Hminus; [lia | simpl].
-                    erewrite nth_error_nil, nth_error_replace_nth' by (simpl in *; lia).
-                    destruct (nth_error_length n0 (removelast a)) as [_ Hnone].
-                    setoid_rewrite Hnone in H2; [auto | lia]. }
-            ++ destruct H3.
-               split.
-               { rewrite replace_nth_length; auto. }
-               intros ?? Hnth.
-               destruct (eq_dec n0 (length (removelast a)));
-                 [|rewrite nth_replace_nth' in Hnth; auto].
-               subst; erewrite nth_replace_nth in Hnth by (simpl in *; lia).
-               inv Hnth.
-               apply H.
-               erewrite app_nth2, minus_diag; auto.
-         -- exists c'; split; auto.
-            erewrite (app_removelast_last None), Ha by auto.
-            apply list_join_filler with (n0 := 1%nat); auto; simpl in *; lia.
-  - split.
-    + split; [eapply list_join_length; eauto|].
-      intros ?? Hnth.
-      apply list_join_nth with (n0 := n) in H.
-      rewrite Hnth in H; inv H; auto.
-      inv H3; auto.
-    + split; [apply join_comm in H; eapply list_join_length; eauto|].
-      intros ?? Hnth.
-      apply list_join_nth with (n0 := n) in H.
-      rewrite Hnth in H; inv H; auto.
-      inv H3; auto.
-  - induction a; unfold list_incl; intros.
-    + destruct b; [constructor|].
-      simpl in *; lia.
-    + destruct H as [? Hnth].
-      destruct b; constructor.
-      * destruct o; [|constructor].
-        specialize (Hnth O _ eq_refl); simpl in Hnth.
-        subst; repeat constructor.
-      * apply IHa.
-        split; [simpl in *; lia|].
-        intros.
-        apply (Hnth (S n)); auto.
-Qed.
-
-Notation union := base.union.
-
-Program Instance set_PCM : Ghost := { valid := fun _ : coPset => True;
-  Join_G a b c := a ## b /\ c = union a b(*; core2 a := empty*) }.
-Next Obligation.
-Proof.
-  exists (fun _ => empty); auto.
-  intro; split; set_solver.
-Defined.
-Next Obligation.
-  constructor.
-    + intros.
-      inv H; inv H0; auto.
-    + intros.
-      inv H; inv H0.
-      eexists; split; [split; eauto | split]; set_solver.
-    + intros.
-      inv H.
-      split; set_solver.
-    + intros.
-      inv H; inv H0.
-      set_solver.
-Qed.
-
-Definition ghost_set g s := own(RA := set_PCM) g s NoneP.
-
-Lemma ghost_set_join : forall g (s1 s2 : coPset),
-  ghost_set g s1 * ghost_set g s2 = !!(s1 ## s2) && ghost_set g (union s1 s2).
-Proof.
-  intros.
-  setoid_rewrite own_op_gen.
-  - instantiate (1 := union s1 s2).
-    unfold ghost_set; apply pred_ext.
-    + Intros; entailer!.
-      destruct H as (? & [] & ?); auto.
-    + Intros; entailer!.
-      eexists; repeat (split; auto).
-  - intros (? & H & ?); inv H; split; auto.
-Qed.
-
-Lemma ghost_set_subset : forall g (s s' : coPset),
-  subseteq s' s -> ghost_set g s = ghost_set g s' * ghost_set g (difference s s').
-Proof.
-  intros.
-  apply own_op.
-  split.
-  - set_solver.
-  - apply union_difference_L; auto.
-Qed.
-
-Corollary ghost_set_remove : forall g a (s : coPset),
-  elem_of a s -> ghost_set g s = ghost_set g (base.singleton a) * ghost_set g (difference s (base.singleton a)).
-Proof.
-  intros; apply ghost_set_subset.
-  set_solver.
-Qed.
-
-Definition iname := nat.
-
-Class invG := { g_inv : gname; g_en : gname; g_dis : gname }.
+Section Invariants.
 
 Context {inv_names : invG}.
 
-Definition master_list {A} g (l : list (option A)) := ghost_master1(ORD := list_order A) l g.
-
-(* up *)
-Instance Inhabitant_option {A} : Inhabitant (option A) := None.
-
-(* Our ghost state construction makes it awkward to put agree inside other ghost state constructions.
-   As a workaround, instead of having one ghost location with a map from indices to agrees,
-   we have a map from indices to ghost locations, each with an agree. *)
-
-Instance token_PCM : Ghost := exclusive_PCM unit.
-
-Definition wsat : mpred := EX I : list mpred, EX lg : list gname, EX lb : list (option bool),
-  !!(length lg = length I /\ length lb = length I) &&
-  master_list g_inv (map (fun i => match Znth i lb with Some _ => Some (Znth i lg)
-                                   | None => None end) (upto (length I))) *
-  ghost_list g_dis (map (fun o => match o with Some true => Some (Some tt) | _ => None end) lb) *
-  ghost_set g_en (list_to_set (map (fun i => Pos.of_nat (S i)) (filter (fun i => decide (nth i lb None = Some false)) (seq 0 (length lb))))) *
-  iter_sepcon (fun i => match Znth i lb with
-                        | Some true => agree (Znth i lg) (Znth i I) * |> Znth i I
-                        | Some false => agree (Znth i lg) (Znth i I)
-                        | _ => emp end) (upto (length I)).
-
-(* This is what's called ownI in Iris; we could build another layer with namespaces. *)
-Definition invariant (i : iname) P : mpred := EX g : gname,
-  ghost_snap(ORD := list_order _) (list_singleton i g) g_inv * agree g P.
-
-Lemma nth_singleton : forall {A} n (a : A) d, nth n (list_singleton n a) d = Some a.
+Lemma invariant_dup : forall i P, invariant i P = invariant i P * invariant i P.
 Proof.
-  intros; unfold list_singleton.
-  rewrite app_nth2; rewrite repeat_length; auto.
-  rewrite minus_diag; auto.
+  exact invariant_dup.
 Qed.
-
-Lemma list_join_singleton_inv : forall {P : Ghost} n a b l,
-  list_join (list_singleton n a) (list_singleton n b) l ->
-  exists c, join a b c /\ l = list_singleton n c.
-Proof.
-  induction n; inversion 1; subst.
-  - inv H5.
-    inv H6; eauto.
-  - edestruct IHn as (c & ? & ?); eauto; subst.
-    inv H5; eauto.
-Qed.
-
-Lemma singleton_join_self : forall {P: Ghost} k (a : G), join a a a ->
-  join (list_singleton k a) (list_singleton k a) (list_singleton k a).
-Proof.
-  intros.
-  rewrite <- (replace_nth_same k (list_singleton k a) None) at 3.
-  rewrite nth_singleton.
-  apply list_join_singleton.
-  + rewrite singleton_length; auto.
-  + rewrite nth_singleton; repeat constructor; auto.
-Qed.
-
-(* not currently useful *)
-(*Global Instance invariant_persistent i P : Persistent (invariant i P).
-Proof.
-  apply bi.exist_persistent; intro.
-  apply bi.sep_persistent; apply own_persistent; hnf; simpl; auto.
-  rewrite !eq_dec_refl; split; auto.
-  apply @singleton_join_self, join_refl.
-Qed.*)
 
 Lemma invariant_cored : forall i P, invariant i P |-- cored.
 Proof.
-  intros; unfold invariant.
-  apply exp_left; intro g.
-  rewrite cored_duplicable.
-  apply sepcon_derives; apply own_cored; hnf; auto; simpl.
-  split; auto.
-  rewrite !eq_dec_refl.
-  apply (singleton_join_self(P := discrete_PCM _)).
-  constructor; auto.
-Qed.
-
-Lemma invariant_dup : forall i P, invariant i P = invariant i P * invariant i P.
-Proof.
-  intros; unfold invariant; apply pred_ext.
-  - Intros g; Exists g g.
-    rewrite <- sepcon_assoc, (sepcon_comm _ (ghost_snap _ _)), <- sepcon_assoc.
-    erewrite ghost_snap_join.
-    erewrite sepcon_assoc, <- agree_dup; apply derives_refl.
-    { apply (singleton_join_self(P := discrete_PCM _)).
-      constructor; auto. }
-  - Intros g1 g2.
-    erewrite <- sepcon_assoc, (sepcon_comm _ (ghost_snap _ _)), <- sepcon_assoc.
-    rewrite ghost_snap_join'; Intros l.
-    apply (list_join_singleton_inv(P := discrete_PCM _)) in H as (g & H & ?); subst.
-    inv H.
-    erewrite sepcon_assoc, <- agree_dup.
-    Exists g; apply derives_refl.
-Qed.
-
-(* up *)
-Lemma Zlength_eq : forall {A B} (l1 : list A) (l2 : list B),
-  Zlength l1 = Zlength l2 <-> length l1 = length l2.
-Proof.
-  intros; rewrite !Zlength_correct.
-  split; [apply Nat2Z.inj|].
-  intro; apply Z2Nat.inj; try lia.
-  rewrite !Nat2Z.id; auto.
-Qed.
-
-Instance list_Perm {P : Ghost} : Perm_alg (list (option G)).
-Proof.
-  apply list_PCM.
-Qed.
-
-(* up *)
-Lemma nth_upto : forall m n d, (n < m)%nat -> nth n (upto m) d = Z.of_nat n.
-Proof.
-  intros.
-  erewrite nth_indep by (rewrite upto_length; auto).
-  erewrite nth_Znth, Znth_upto; auto.
-  split; [lia|].
-  apply Nat2Z.inj_lt; auto.
-Qed.
-
-Lemma nth_repeat : forall {A} n m (a : A), nth n (repeat a m) a = a.
-Proof.
-  induction n; destruct m; simpl; auto.
-Qed.
-
-Lemma list_incl_singleton : forall {A} n (a : A) l,
-  list_incl (list_singleton n a) l <-> nth n l None = Some a.
-Proof.
-  unfold list_incl; split.
-  - intros [? Hnth].
-    apply Hnth.
-    rewrite nth_singleton; auto.
-  - intros; split.
-    + rewrite singleton_length.
-      destruct (lt_dec n (length l)); [lia|].
-      erewrite nth_overflow in H by lia; discriminate.
-    + intros ??.
-      unfold list_singleton.
-      destruct (lt_dec n0 n).
-      * erewrite app_nth1 by (rewrite repeat_length; auto).
-        rewrite nth_repeat; discriminate.
-      * rewrite app_nth2; rewrite repeat_length; try lia.
-        destruct (eq_dec n0 n); [|erewrite nth_overflow by (simpl; lia); discriminate].
-        subst; rewrite minus_diag; simpl.
-        intro X; inv X; auto.
-Qed.
-
-Lemma seq_app : forall a b c, seq a (b + c) = seq a b ++ seq (a + b) c.
-Proof.
-  intros ??; revert a; induction b; simpl; intros; auto.
-  rewrite IHb; do 3 f_equal; omega.
-Qed.
-
-Lemma filter_ext_in : forall {A} (f g : A -> bool) l, (forall x, In x l -> f x = g x) -> filter f l = filter g l.
-Proof.
-  induction l; auto; simpl; intros.
-  rewrite -> H by auto.
-  rewrite IHl; auto.
-Qed.
-
-Lemma filter_none : forall {A} (f : A -> bool) l, (forall x, In x l -> f x = false) -> filter f l = [].
-Proof.
-  induction l; auto; simpl; intros.
-  rewrite H; auto.
+  exact invariant_cored.
 Qed.
 
 Lemma wsat_alloc : forall P, (wsat * |> P |-- |==> wsat * EX i : _, invariant i P)%I.
@@ -834,29 +146,26 @@ Proof.
   - iExists ((l ++ repeat emp i) ++ [P]), ((lg ++ repeat O i) ++ [g]),
          ((lb ++ repeat None i) ++ [Some true]).
     erewrite !(app_length (_ ++ _)); simpl.
-    erewrite upto_app, iter_sepcon_app; simpl.
+    erewrite !iter_sepcon_eq, upto_app, iter_sepcon_app; simpl.
     erewrite Z.add_0_r, <- Zlength_correct, !app_Znth2; erewrite !Zlength_app, !Zlength_repeat; try lia.
     erewrite Hlg, Hlb, Zminus_diag, !Znth_0_cons.
-    erewrite prop_true_andp by (erewrite !app_length, !repeat_length; lia).
+    erewrite predicates_hered.prop_true_andp by (erewrite !app_length, !repeat_length; lia).
     iFrame.
     iSplitL "en".
-    + rewrite app_length -plus_assoc seq_app filter_app.
-      rewrite (filter_none _ (seq _ (_ + 1))).
-      rewrite app_nil_r.
-      erewrite filter_ext_in; auto.
-      * intros ??%in_seq; simpl.
-        rewrite <- app_assoc, app_nth1 by lia; auto.
-      * intros ??%in_seq; simpl.
-        rewrite <- app_assoc, app_nth2 by lia.
-        destruct (lt_dec (x - length lb) i); [rewrite app_nth1 | rewrite app_nth2];
-          rewrite ?repeat_length; try lia.
-        -- rewrite nth_repeat; auto.
-        -- destruct (x - length lb - i)%nat; auto; simpl.
-          destruct n0; auto.
+    + erewrite Ensembles.Extensionality_Ensembles at 1; [iApply "en"|].
+      constructor; intros ? X; unfold Ensembles.In in *.
+      * destruct (lt_dec x (length lb)).
+      rewrite !app_nth app_length.
+      destruct (lt_dec _ _); [|omega].
+      destruct (lt_dec _ _); [auto | omega].
+      { rewrite -> nth_overflow in X by omega; discriminate. }
+      * rewrite !app_nth nth_repeat in X.
+      repeat destruct (lt_dec _ _); auto; try discriminate.
+      destruct (x - _)%nat; [|destruct n0]; inv X.
     + erewrite app_length, upto_app, iter_sepcon_app.
       rewrite <- sepcon_emp at 1; iDestruct "I" as "[I emp]".
       iSplitL "I".
-      * erewrite iter_sepcon_func_strong; auto.
+      * erewrite iter_sepcon_func_strong; [iApply "I"|].
         intros ??%In_upto.
         rewrite <- Zlength_correct in *.
         rewrite <- !app_assoc, !app_Znth1 by (rewrite ?Zlength_app; lia); auto.
@@ -871,16 +180,10 @@ Proof.
     iExists g; rewrite H; iFrame.
 Qed.
 
-Lemma list_to_set_eq : forall (l1 l2 : list positive), (forall x, elem_of x l1 <-> elem_of x l2) ->
-  (list_to_set l1 : coPset) = list_to_set l2.
-Proof.
-  intros.
-  apply coPset_leibniz, elem_of_equiv; intros.
-  rewrite !elem_of_list_to_set; auto.
-Qed.
+Existing Instance token_PCM.
 
 Lemma wsat_open : forall i P,
-  (wsat * invariant i P * ghost_set g_en (base.singleton (Pos.of_nat (S i))) |--
+  (wsat * invariant i P * ghost_set g_en (Ensembles.Singleton _ i) |--
   |==> wsat * |> P * ghost_list g_dis (list_singleton i (Some tt)))%I.
 Proof.
   intros; unfold wsat, invariant.
@@ -898,46 +201,39 @@ Proof.
   iMod (@own_dealloc (snap_PCM(ORD := list_order _)) with "snap").
   iModIntro.
   destruct Hi as (? & ? & b & Hi).
-  assert (nth i lb None = Some b) as Hi' by (rewrite <- nth_Znth in Hi; auto).
+  assert (nth i lb None = Some b) as Hi' by (rewrite <- nth_Znth' in Hi; auto).
   destruct b.
   erewrite ghost_list_nth with (n := i) by (erewrite nth_map' with (d' := None), Hi'; eauto; lia).
   iDestruct "dis" as "[token dis]".
-  erewrite iter_sepcon_Znth with (i0 := Z.of_nat i)
+  rewrite -> iter_sepcon_eq, iter_sepcon_Znth with (i0 := Z.of_nat i)
     by (rewrite Zlength_upto; split; [|apply Nat2Z.inj_lt]; lia).
   erewrite Znth_upto, Hi by lia.
   iDestruct "I" as "((agree' & HP) & I)".
   subst; iDestruct (agree_join with "[agree agree']") as "[imp agree]"; first iFrame.
-  iSplitR "token"; last auto.
-  iSplitR "HP imp"; last (iApply "imp"; auto).
+  iSplitR "token"; last iFrame.
+  iSplitR "HP imp"; last (iApply "imp"; iFrame).
   iExists l, lg, (replace_nth i lb (Some false)).
-  rewrite replace_nth_length prop_true_andp; last auto.
+  rewrite replace_nth_length predicates_hered.prop_true_andp; last auto.
   iSplitR "I agree".
   iSplitR "en en1".
   iSplitR "dis".
-  - erewrite map_ext; eauto.
+  - erewrite map_ext; [iFrame|].
     intros; simpl.
     destruct (eq_dec a (Z.of_nat i)); [subst; rewrite Znth_replace_nth | rewrite Znth_replace_nth'];
       auto; try lia.
     rewrite Hi; auto.
-  - rewrite map_replace_nth; auto.
+  - rewrite map_replace_nth; iFrame.
   - iCombine "en en1" as "en"; erewrite ghost_set_join.
     iDestruct "en" as "[% en]".
-    erewrite coPset_leibniz; auto; split.
-    + intros Hin%elem_of_union; rewrite -> elem_of_list_to_set, elem_of_list_In, in_map_iff in *; destruct Hin as [Hin | Hin].
-      * destruct Hin as (x' & ? & Hin); subst.
-        apply filter_In in Hin as [Hin ?].
-        do 2 eexists; eauto; apply filter_In; split; auto.
-        destruct (decide (x' = i)); [subst; rewrite nth_replace_nth | rewrite nth_replace_nth']; auto; lia.
-      * apply elem_of_singleton in Hin; subst.
-        do 2 eexists; eauto; apply filter_In.
-        split; [|rewrite nth_replace_nth; auto; lia].
-        apply in_seq; lia.
-    + intros Hin; rewrite elem_of_union; rewrite -> elem_of_list_to_set, elem_of_list_In, in_map_iff in *.
-      destruct Hin as (x' & ? & Hin); subst.
-      destruct (decide (x' = i)); [subst; rewrite elem_of_singleton; auto|].
-      left; do 2 eexists; eauto.
-      apply filter_In in Hin as [Hin ?]; rewrite filter_In; split; auto.
-      erewrite nth_replace_nth' in H2; auto.
+    erewrite Ensembles.Extensionality_Ensembles at 1; [iFrame | constructor; intros ? X].
+    + destruct (eq_dec x i).
+      * subst; unfold Ensembles.In; apply nth_replace_nth; omega.
+      * inv X; unfold Ensembles.In in *.
+        rewrite nth_replace_nth'; auto.
+        { inv H2; contradiction. }
+    + destruct (eq_dec x i); [subst; right; constructor | left].
+      unfold Ensembles.In in *.
+      rewrite nth_replace_nth' in X; auto.
   - erewrite iter_sepcon_Znth with (i0 := Z.of_nat i)(l0 := upto _)
       by (rewrite Zlength_upto; split; [|apply Nat2Z.inj_lt]; lia).
     erewrite Znth_upto, Znth_replace_nth by lia; iFrame.
@@ -948,13 +244,8 @@ Proof.
     apply in_app in Hin as [?%In_sublist_upto | ?%In_sublist_upto]; lia.
   - iCombine "en en1" as "en"; erewrite ghost_set_join.
     iDestruct "en" as "[% en]".
-    rewrite -> elem_of_disjoint in H2.
-    contradiction (H2 (Pos.of_nat (S i))).
-    + rewrite -> elem_of_list_to_set, elem_of_list_In, in_map_iff.
-      do 2 eexists; eauto.
-      rewrite filter_In; split; [|rewrite Hi'; auto].
-      apply in_seq; lia.
-    + apply elem_of_singleton; auto.
+    inv H2.
+    contradiction (H3 i); constructor; auto; constructor.
 Qed.
 
 (* up *)
@@ -965,7 +256,7 @@ Qed.
 
 Lemma wsat_close : forall i P,
   (wsat * invariant i P * |> P * ghost_list g_dis (list_singleton i (Some tt)) |--
-  |==> wsat * ghost_set g_en (base.singleton (Pos.of_nat (S i))))%I.
+  |==> wsat * ghost_set g_en (Ensembles.Singleton _ i))%I.
 Proof.
   intros; unfold wsat, invariant.
   iIntros "(((H & inv1) & HP) & dis1)". iDestruct "H" as (l lg lb) "((((% & inv) & dis) & en) & I)". iDestruct "inv1" as (g) "[snap agree]".
@@ -982,7 +273,7 @@ Proof.
   iMod (@own_dealloc (snap_PCM(ORD := list_order _)) with "snap").
   iModIntro.
   destruct Hi as (? & ? & b & Hi).
-  assert (nth i lb None = Some b) as Hi' by (rewrite <- nth_Znth in Hi; auto).
+  assert (nth i lb None = Some b) as Hi' by (rewrite <- nth_Znth' in Hi; auto).
   destruct b.
   { iCombine "dis dis1" as "dis".
     iDestruct (own_valid_2(RA := list_PCM _) with "dis") as %H2.
@@ -992,41 +283,36 @@ Proof.
     rewrite Hi' in J; inv J.
     inv H5.
     inv H3. }
-  erewrite ghost_set_remove with (a := Pos.of_nat (S i)).
+  erewrite ghost_set_remove with (a := i).
   iDestruct "en" as "[$ en]".
   iExists l, lg, (replace_nth i lb (Some true)).
-  rewrite replace_nth_length prop_true_andp; last auto.
+  rewrite replace_nth_length predicates_hered.prop_true_andp; last auto.
   iSplitR "I agree HP".
   iSplitR "en".
   iSplitR "dis dis1".
-  - erewrite map_ext; eauto.
+  - erewrite map_ext; [iFrame|].
     intros.
     destruct (eq_dec a (Z.of_nat i)); [subst; rewrite Znth_replace_nth | rewrite Znth_replace_nth'];
       auto; try lia.
     rewrite Hi; auto.
-  - iCombine "dis1 dis" as "dis"; setoid_rewrite <- own_op; auto.
+  - iCombine "dis1 dis" as "dis"; setoid_rewrite <- own.ghost_op; [iFrame|].
     rewrite map_replace_nth.
     apply (list_join_singleton(P := token_PCM)).
     { rewrite map_length; lia. }
     erewrite nth_map' with (d' := None) by lia.
     rewrite Hi'; constructor.
-  - erewrite coPset_leibniz; auto; split.
-    + rewrite -> elem_of_difference, !elem_of_list_to_set, !elem_of_list_In, !in_map_iff.
-      intros ((? & ? & Hin) & Hout); subst.
-      do 2 eexists; eauto.
-      rewrite -> filter_In in *; destruct Hin; split; auto.
+  - erewrite Ensembles.Extensionality_Ensembles at 1; [iFrame|]; constructor; intros ? X.
+    + inv X; unfold Ensembles.In in *.
       rewrite nth_replace_nth'; auto.
-      intro; subst; contradiction Hout; apply elem_of_singleton; auto.
-    + rewrite -> elem_of_difference, !elem_of_list_to_set, !elem_of_list_In, !in_map_iff.
-      intros (x' & ? & Hin) ; subst.
-      rewrite -> filter_In in *; destruct Hin as [? Hin].
-      destruct (decide (x' = i)); [subst; erewrite nth_replace_nth in Hin by lia; discriminate|].
-      erewrite nth_replace_nth' in Hin by auto.
-      split; [|rewrite elem_of_singleton; auto].
-      do 2 eexists; eauto.
-      rewrite filter_In; split; auto.
-      intros X%Nat2Pos.inj; congruence.
-  - erewrite iter_sepcon_Znth with (i0 := Z.of_nat i)
+      intro; subst; contradiction.
+    + constructor.
+      * unfold Ensembles.In in *.
+        destruct (eq_dec x i); [subst; auto|].
+        rewrite nth_replace_nth' in X; auto.
+      * intro X'; inv X'.
+        unfold Ensembles.In in X.
+        rewrite -> nth_replace_nth in X by omega; inv X.
+  - erewrite !iter_sepcon_eq, iter_sepcon_Znth with (i0 := Z.of_nat i)
       by (rewrite Zlength_upto; split; [|apply Nat2Z.inj_lt]; lia).
     erewrite iter_sepcon_Znth with (i0 := Z.of_nat i)(l0 := upto _)
       by (rewrite Zlength_upto; split; [|apply Nat2Z.inj_lt]; lia).
@@ -1040,48 +326,16 @@ Proof.
     rewrite Znth_replace_nth'; auto.
     intro; subst.
     apply in_app in Hin as [?%In_sublist_upto | ?%In_sublist_upto]; lia.
-  - rewrite -> elem_of_list_to_set, elem_of_list_In, in_map_iff.
-    do 2 eexists; eauto.
-    rewrite filter_In; split; [|rewrite Hi'; auto].
-    apply in_seq; lia.
+  - unfold Ensembles.In; auto.
 Qed.
 
 Lemma invariant_dealloc : forall i P, (invariant i P |-- |==> emp)%I.
 Proof.
-  intros; unfold invariant.
-  Intro g.
-  rewrite <- (emp_sepcon emp%I).
-  eapply derives_trans, bupd_sep.
-  apply sepcon_derives; apply own_dealloc.
-Qed.
-
-Lemma invariant_super_non_expansive : forall n N P,
-  approx n (invariant N P) = approx n (invariant N (approx n P)).
-Proof.
-  intros; unfold invariant.
-  rewrite !approx_exp; f_equal; extensionality g.
-  rewrite !approx_sepcon; f_equal.
-  apply own_super_non_expansive.
+  exact invariant_dealloc.
 Qed.
 
 (* Consider putting rules for invariants and fancy updates in msl (a la ghost_seplog), and proofs
    in veric (a la own). *)
-
-Lemma ghost_set_empty : forall g s,
-  ghost_set g s = ghost_set g s * ghost_set g empty.
-Proof.
-  intros.
-  apply own_op.
-  hnf; set_solver.
-Qed.
-
-Lemma wsat_empty_eq : wsat = wsat * ghost_set g_en empty.
-Proof.
-  unfold wsat.
-  repeat (rewrite exp_sepcon1; f_equal; extensionality).
-  erewrite ghost_set_empty at 1.
-  apply pred_ext; entailer!.
-Qed.
 
 End Invariants.
 
@@ -1094,5 +348,5 @@ Proof.
   iMod (own_alloc(RA := set_PCM) empty NoneP with "[$]") as (g_en) "en"; first (simpl; auto).
   iModIntro.
   iExists {| g_inv := g_inv; g_dis := g_dis; g_en := g_en |}.
-  iExists nil, nil, nil; simpl; iFrame; auto.
+  iExists nil, nil, nil; simpl; iFrame "inv dis en"; auto.
 Qed.
