veric/bi.v
@@ -407,5 +407,179 @@ Proof.
 Qed.
 Global Instance mpred_bi_bupd : BiBUpd mpredI := {| bi_bupd_mixin := mpred_bupd_mixin |}.
 
+(*(* Lifted instance *)
+Section lifted_cofe.
+  Instance env_mpred_equiv : Equiv (environ -> mpred) := eq.
+  Instance env_mpred_dist : Dist (environ -> mpred) := fun n P Q => forall rho, approx (S n) (P rho) = approx (S n) (Q rho).
+
+  Lemma lift_dist_equiv : forall (P Q : environ -> pred rmap), (∀ n : nat, P ≡{n}≡ Q) -> P = Q.
+  Proof.
+    intros; extensionality rho.
+    apply dist_equiv; intros.
+    apply H.
+  Qed.
+
+  Definition env_mpred_ofe_mixin : OfeMixin (environ -> mpred).
+  Proof.
+    split.
+    - intros P Q; split.
+      + intros HPQ n; hnf in *; subst; auto.
+      + apply lift_dist_equiv.
+    - intros n; constructor; repeat intro; auto.
+      congruence.
+    - intros ? P Q ? rho.
+      apply (mixin_dist_S _ mpred_ofe_mixin), H.
+  Qed.
+  Canonical Structure env_mpredC : ofeT := OfeT (environ -> mpred) env_mpred_ofe_mixin.
+
+  Program Definition env_mpred_compl : Compl env_mpredC := fun c rho w => c (level w) rho w.
+  Next Obligation.
+  Proof.
+    repeat intro.
+    eapply pred_hereditary in H0; eauto.
+    assert (approx (S (level a')) (c (level a) rho) a') as Ha by (split; auto).
+    rewrite chain_cauchy in Ha; [apply Ha | apply age_level in H; lia].
+  Qed.
+  Global Program Instance env_mpred_cofe : Cofe env_mpredC := {| compl := env_mpred_compl |}.
+  Next Obligation.
+    intros; hnf; intro rho.
+    apply predicates_hered.pred_ext; intros ? []; split; auto; simpl in *.
+    - assert (approx (S (level a)) (c (level a) rho) a) as Ha by (split; auto).
+      rewrite <- (chain_cauchy c (level a) n) in Ha; [apply Ha | lia].
+    - assert (approx (S (level a)) (c n rho) a) as Ha by (split; auto).
+      rewrite chain_cauchy in Ha; [apply Ha | lia].
+  Qed.
+End lifted_cofe.
+Arguments env_mpredC : clear implicits.
+
+Lemma env_mpred_bi_mixin :
+  BiMixin(PROP := environ -> mpred)
+    derives emp prop andp orp imp (@allp _ _) (@exp _ _) sepcon wand (lift persistently).
+Proof.
+  split.
+  - constructor; auto. intro. apply derives_trans.
+  - split; intros.
+    + hnf in H; subst; auto.
+    + apply pred_ext; tauto.
+  - intros ????; hnf; intro rho.
+    f_equal; f_equal.
+    apply prop_ext; auto.
+  - intros ????????; hnf in *.
+    rewrite !approx_andp; congruence.
+  - intros ????????; hnf in *.
+    rewrite !approx_orp; congruence.
+  - intros ????????; hnf in *; simpl.
+    rewrite approx_imp (approx_imp _ (y rho)). congruence.
+  - intros ?? P Q ??; hnf in *; simpl.
+    apply (bi_mixin_forall_ne _ _ _ _ _ _ _ _ _ _ _ mpred_bi_mixin); hnf; intros.
+    apply H.
+  - intros ?? P Q ??; hnf in *.
+    rewrite !approx_exp; f_equal; extensionality.
+    apply H.
+  - intros ????????; hnf in *.
+    rewrite !approx_sepcon; congruence.
+  - intros ? P Q ?????; hnf in *; simpl.
+    rewrite wand_nonexpansive (wand_nonexpansive (Q rho)); congruence.
+  - intros ?????; hnf in *.
+    unfold lift.
+    rewrite !approx_persistently H; auto.
+  - apply prop_right.
+  - intros.
+    apply prop_left; intro.
+    eapply derives_trans; eauto.
+  - intros; rewrite prop_forall; auto.
+  - intros; apply andp_left1, derives_refl.
+  - intros; apply andp_left2, derives_refl.
+  - intros; apply andp_right; auto.
+  - intros; apply orp_right1, derives_refl.
+  - intros; apply orp_right2, derives_refl.
+  - apply orp_left.
+  - apply imp_andp_adjoint.
+  - apply imp_andp_adjoint.
+  - intros; apply allp_right; auto.
+  - intros; eapply allp_left, derives_refl.
+  - intros; eapply exp_right, derives_refl.
+  - intros; apply exp_left; auto.
+  - intros; apply sepcon_derives; auto.
+  - intros; rewrite emp_sepcon; auto.
+  - intros; rewrite emp_sepcon; auto.
+  - intros; rewrite sepcon_comm; auto.
+  - intros; rewrite sepcon_assoc; auto.
+  - intros; rewrite <- wand_sepcon_adjoint; auto.
+  - intros; rewrite wand_sepcon_adjoint; auto.
+  - intros; unfold lift; simpl.
+    intro; apply persistently_derives; auto.
+  - intros; unfold lift; simpl.
+    intro; apply persistently_persists.
+  - unfold persistently, lift; intro rho.
+    unseal_derives; intros ??; simpl.
+    apply core_identity.
+  - intros; intro rho.
+    unfold lift; simpl; apply (bi_mixin_persistently_forall_2 _ _ _ _ _ _ _ _ _ _ _ mpred_bi_mixin).
+  - intros; intro rho.
+    unfold lift; simpl; apply (bi_mixin_persistently_exist_1 _ _ _ _ _ _ _ _ _ _ _ mpred_bi_mixin).
+  - intros; intro rho.
+    unfold lift; simpl; apply (bi_mixin_persistently_absorbing _ _ _ _ _ _ _ _ _ _ _ mpred_bi_mixin).
+  - intros; intro rho.
+    unfold lift; simpl; apply (bi_mixin_persistently_and_sep_elim _ _ _ _ _ _ _ _ _ _ _ mpred_bi_mixin).
+Qed.
+
+Lemma env_mpred_sbi_mixin : SbiMixin(PROP := environ -> mpred)
+  derives prop orp imp (@allp _ _) (@exp _ _) sepcon (lift persistently) (fun a b c _ => @internal_eq a b c) seplog.later.
+Proof.
+  split.
+  - repeat intro; hnf.
+    simpl; apply (sbi_mixin_later_contractive _ _ _ _ _ _ _ _ _ _ mpred_sbi_mixin).
+    destruct n; simpl in *; hnf; auto.
+  - repeat intro; apply (sbi_mixin_internal_eq_ne _ _ _ _ _ _ _ _ _ _ mpred_sbi_mixin); auto.
+  - intros; intro rho.
+    apply (sbi_mixin_internal_eq_refl _ _ _ _ _ _ _ _ _ _ mpred_sbi_mixin).
+  - intros; intro rho; simpl.
+    match goal with |- ?P |-- (?A --> ?B)%logic =>
+      change (predicates_hered.derives P (predicates_hered.imp A B)) end.
+    repeat intro; simpl in *.
+    assert ((approx (S (level a')) (Ψ b rho)) a') as []; auto.
+    rewrite <- H; [split; eauto|].
+    eapply dist_le; eauto.
+    apply necR_level in H1; lia.
+  - intros; intro rho.
+    unseal_derives; repeat intro.
+    specialize (H x); auto.
+  - intros; intro rho.
+    unseal_derives; repeat intro.
+    apply H.
+  - intros; intro rho.
+    unseal_derives; repeat intro; simpl in *.
+    rewrite discrete_iff; apply H0.
+  - intros; intro rho.
+    apply (sbi_mixin_later_eq_1 _ _ _ _ _ _ _ _ _ _ mpred_sbi_mixin).
+  - intros; intro rho.
+    apply (sbi_mixin_later_eq_2 _ _ _ _ _ _ _ _ _ _ mpred_sbi_mixin).
+  - intros; apply later_derives; auto.
+  - apply now_later.
+  - intros. rewrite seplog.later_allp; auto.
+  - intros. eapply derives_trans; [eapply (seplog.later_exp'')|].
+    apply orp_left; [apply orp_right2 | apply orp_right1]; auto.
+    apply later_derives, FF_left.
+  - intros; rewrite later_sepcon; auto.
+  - intros; rewrite later_sepcon; auto.
+  - intros; intro rho; unfold lift; simpl.
+    apply (sbi_mixin_later_persistently_1 _ _ _ _ _ _ _ _ _ _ mpred_sbi_mixin).
+  - intros; intro rho; unfold lift; simpl.
+    apply (sbi_mixin_later_persistently_2 _ _ _ _ _ _ _ _ _ _ mpred_sbi_mixin).
+  - intros; intro rho; unfold lift; simpl.
+    apply (sbi_mixin_later_false_em _ _ _ _ _ _ _ _ _ _ mpred_sbi_mixin).
+Qed.
+
+Canonical Structure env_mpredI : bi :=
+  {| bi_ofe_mixin := env_mpred_ofe_mixin; bi_bi_mixin := env_mpred_bi_mixin |}.
+Canonical Structure env_mpredSI : sbi :=
+  {| sbi_ofe_mixin := env_mpred_ofe_mixin;
+     sbi_bi_mixin := env_mpred_bi_mixin; sbi_sbi_mixin := env_mpred_sbi_mixin |}.*)
+
+(* Return from IPM to VST entailment. *)
+Ltac iVST := iStopProof; match goal with |-bi_entails ?P ?Q => change (P |-- Q) end;
+  repeat match goal with |-context[bi_sep ?P ?Q] => change (bi_sep P Q) with (P * Q) end.
+
 Open Scope Z.
 Open Scope logic.
