veric/ghosts.v
@@ -1,0 +1,552 @@
+Require Export VST.msl.ghost.
+Require Import VST.msl.shares.
+Require Import VST.msl.sepalg_generators.
+Require Import VST.msl.iter_sepcon.
+Require Import VST.msl.ghost_seplog.
+Require Import VST.veric.mpred.
+Require Import VST.veric.shares.
+Require Import VST.veric.own.
+Require Import VST.veric.compcert_rmaps.
+
+(* Lemmas about ghost state and common instances *)
+
+Notation "|==> P" := (own.bupd P) (at level 99, P at level 200): pred.
+
+Section ghost.
+
+Local Open Scope pred.
+
+Context {RA: Ghost}.
+
+Lemma own_op' : forall g a1 a2 pp,
+  own g a1 pp * own g a2 pp = EX a3 : _, !!(join a1 a2 a3 /\ valid a3) && own g a3 pp.
+Proof.
+  intros.
+  apply pred_ext.
+  - eapply derives_trans, prop_andp_left; [apply andp_right, derives_refl; apply ghost_valid_2|].
+    intros (a3 & ? & ?); apply exp_right with a3, prop_andp_right; auto.
+    erewrite <- ghost_op by eauto; apply derives_refl.
+  - apply exp_left; intro; apply prop_andp_left; intros [].
+    erewrite ghost_op by eauto; apply derives_refl.
+Qed.
+
+Lemma own_op_gen : forall g a1 a2 a3 pp, (valid_2 a1 a2 -> join a1 a2 a3) ->
+  own g a1 pp * own g a2 pp = !!(valid_2 a1 a2) && own g a3 pp.
+Proof.
+  intros; apply pred_ext.
+  - eapply derives_trans, prop_andp_left; [apply andp_right, derives_refl; apply ghost_valid_2|].
+    intro; erewrite <- ghost_op by eauto.
+    apply prop_andp_right; auto.
+  - apply prop_andp_left; intro.
+    erewrite ghost_op by eauto; apply derives_refl.
+Qed.
+
+End ghost.
+
+Hint Resolve Share.nontrivial : share.
+ 
+Section Reference.
+(* One common kind of PCM is one in which a central authority has a reference copy, and clients pass around
+   partial knowledge. When a client recovers all pieces, it can gain full knowledge. *)
+(* This is related to the snapshot PCM, but the snapshots aren't duplicable. *)
+
+Lemma join_Bot : forall a b, sepalg.join a b Share.bot -> a = Share.bot /\ b = Share.bot.
+Proof.
+  intros ?? (? & ?).
+  apply lub_bot_e; auto.
+Qed.
+
+Global Program Instance pos_PCM (P : Ghost) : Ghost := { G := option (share * G);
+  valid a := match a with Some (sh, _) => sh <> Share.bot | _ => True end;
+  Join_G a b c := match a, b, c with
+  | Some (sha, a'), Some (shb, b'), Some (shc, c') =>
+      sha <> Share.bot /\ shb <> Share.bot /\ sepalg.join sha shb shc /\ join a' b' c'
+  | Some (sh, a), None, Some c' | None, Some (sh, a), Some c' => c' = (sh, a)
+  | None, None, None => True
+  | _, _, _ => False
+  end(*;
+  core2 a := None*) }.
+Next Obligation.
+repeat split; intros; intro X; decompose [and] X; congruence.
+Qed.
+Next Obligation.
+repeat split; intros; intro X; decompose [and] X; congruence.
+Qed.
+Next Obligation.
+repeat split; intros; intro X; decompose [and] X; congruence.
+Qed.
+Next Obligation.
+repeat split; intros; intro X; decompose [and] X; congruence.
+Qed.
+Next Obligation.
+exists (fun _ => None); auto.
+intros [[]|]; constructor.
+Defined.
+Next Obligation.
+constructor.
+  - intros [[]|] [[]|] [[]|] [[]|]; unfold join; simpl; auto; try contradiction; try congruence.
+    intros (? & ? & ? & ?) (? & ? & ? & ?); f_equal; f_equal; eapply join_eq; eauto.
+  - intros [[]|] [[]|] [[]|] [[]|] [[]|]; try contradiction; unfold join; simpl;
+      intros; decompose [and] H; decompose [and] H0;
+      repeat match goal with H : (_, _) = (_, _) |- _ => inv H end;
+      try solve [eexists (Some _); split; auto; simpl; auto]; try solve [exists None; split; auto].
+    + destruct (join_assoc H2 H6) as (sh' & ? & ?), (join_assoc H5 H9) as (a' & ? & ?).
+      exists (Some (sh', a')); repeat (split; auto).
+      intro; subst.
+      apply join_Bot in H8 as []; auto.
+    + exists (Some (s2, g2)); auto.
+  - intros [[]|] [[]|] [[]|]; try contradiction; unfold join; auto.
+    intros (? & ? & ? & ?); split; auto; split; auto; split; apply join_comm; auto.
+  - intros [[]|] [[]|] [[]|] [[]|]; try contradiction; intros H1 H2; try solve [inv H1; reflexivity || inv H2; reflexivity].
+    destruct H1 as (? & ? & ? & ?), H2 as (? & ? & ? & ?); f_equal; f_equal; eapply join_positivity; eauto.
+Qed.
+(*Next Obligation.
+  hnf.
+  destruct a as [[]|]; auto.
+Qed.
+Next Obligation.
+  exists None; hnf; auto.
+Qed.*)
+Next Obligation.
+destruct a as [[]|]; destruct b as [[]|]; destruct c as [[]|]; try trivial;
+unfold join in *; try contradiction.
+- decompose [and] H; assumption.
+- congruence.
+Qed.
+
+Definition completable {P : Ghost} (a: @G (pos_PCM P)) r := exists x, join a x (Some (Share.top, r)).
+
+Local Obligation Tactic := idtac.
+
+Global Program Instance ref_PCM (P : Ghost) : Ghost :=
+{ valid a := valid (fst a) /\ match snd a with Some r => completable (fst a) r | None => True end;
+  Join_G a b c := @Join_G (pos_PCM P) (fst a) (fst b) (fst c) /\
+    @psepalg.Join_lower _ (psepalg.Join_discrete _) (snd a) (snd b) (snd c)(*;
+  core2 a := (None, None)*) }.
+Next Obligation.
+  intros P; apply sepalg_generators.Sep_prod.
+  + apply @Sep_G.
+  + apply psepalg.Sep_option.
+Defined.
+Next Obligation.
+  intros P; apply sepalg_generators.Perm_prod.
+  + apply @Perm_G.
+  + apply psepalg.Perm_option.
+Qed.
+(*Next Obligation.
+  intros; hnf.
+  split; [apply (@core2_unit (pos_PCM P)) | constructor].
+Qed.
+Next Obligation.
+  intros; reflexivity.
+Qed.
+Next Obligation.
+  intros; exists (None, None); hnf.
+  split; constructor.
+Qed.*)
+Next Obligation.
+  intros P ??? [? J] []; split; [eapply join_valid; eauto|].
+  destruct a, b, c; simpl in *; inv J; auto.
+  + destruct o1; auto.
+    destruct H1.
+    destruct (join_assoc H H1) as (? & ? & ?); eexists; eauto.
+  + inv H2.
+Qed.
+
+End Reference.
+
+Program Instance exclusive_PCM A : Ghost :=
+  { valid a := True; Join_G := Join_lower (Join_discrete A)(*; core2 a := None*) }.
+(*Next Obligation.
+Proof.
+  eexists; constructor.
+Qed.*)
+
+Definition excl {A} g a : mpred := own(RA := exclusive_PCM A) g (Some a) NoneP.
+
+Lemma exclusive_update : forall {A} (v v' : A) p, excl p v |-- |==> excl p v'.
+Proof.
+  intros; apply ghost_update.
+  intros ? (? & ? & _).
+  exists (Some v'); split; simpl; auto; inv H; constructor.
+  inv H1.
+Qed.
+
+Local Obligation Tactic := idtac.
+
+Program Instance prod_PCM (GA GB: Ghost): Ghost := { G := @G GA * @G GB;
+  valid a := valid (fst a) /\ valid (snd a); Join_G := Join_prod _ _ _ _ }.
+Next Obligation.
+  intros GA GB ??? [] []; split; eapply join_valid; eauto.
+Defined.
+
+(* Can we use Santiago and Qinxiang's paper to simplify this? *)
+Class PCM_order `{P : Ghost} (ord : G -> G -> Prop) := { ord_preorder :> PreOrder ord;
+  ord_lub : forall a b c, ord a c -> ord b c -> {c' | join a b c' /\ ord c' c};
+  join_ord : forall a b c, join a b c -> ord a c /\ ord b c; ord_join : forall a b, ord b a -> join a b a }.
+
+(*Class lub_ord {A} (ord : A -> A -> Prop) := { lub_ord_refl :> RelationClasses.Reflexive ord;
+  lub_ord_trans :> RelationClasses.Transitive ord;
+  has_lub : forall a b c, ord a c -> ord b c -> exists c', ord a c' /\ ord b c' /\
+    forall d, ord a d -> ord b d -> ord c' d }.
+
+Global Instance ord_PCM `{lub_ord} : Ghost := { Join_G a b c := ord a c /\ ord b c /\
+  forall c', ord a c' -> ord b c' -> ord c c' }.
+Proof.
+  - 
+  - intros ??? (? & ? & ?); eauto.
+  - intros ????? (? & ? & Hc) (? & ? & He).
+    destruct (has_lub b d e) as (c' & ? & ? & Hlub); try solve [etransitivity; eauto].
+    exists c'; repeat split; auto.
+    + etransitivity; eauto.
+    + apply Hlub; auto; transitivity c; auto.
+    + intros.
+      apply He.
+      * apply Hc; auto; etransitivity; eauto.
+      * etransitivity; eauto.
+Defined.
+
+Global Instance ord_PCM_ord `{lub_ord} : PCM_order ord.
+Proof.
+  constructor.
+  - apply lub_ord_refl.
+  - apply lub_ord_trans.
+  - intros ??? Ha Hb.
+    destruct (has_lub _ _ _ Ha Hb) as (c' & ? & ? & ?).
+    exists c'; simpl; eauto.
+  - simpl; intros; tauto.
+  - intros; simpl.
+    repeat split; auto.
+    reflexivity.
+Defined.*)
+
+(* Instances of ghost state *)
+Section Snapshot.
+(* One common kind of PCM is one in which a central authority has a reference copy, and clients pass around
+   partial knowledge. *)
+
+Context `{ORD : PCM_order}.
+
+Lemma join_refl : forall (v : G), join v v v.
+Proof.
+  intros. apply ord_join; reflexivity.
+Qed.
+
+Lemma join_compat : forall v1 v2 v' v'', join v2 v' v'' -> ord v1 v2 -> exists v0, join v1 v' v0 /\ ord v0 v''.
+Proof.
+  intros.
+  destruct (join_ord _ _ _ H).
+  destruct (ord_lub v1 v' v'') as (? & ? & ?); eauto.
+  etransitivity; eauto.
+Qed.
+
+Lemma join_ord_eq : forall a b, ord a b <-> exists c, join a c b.
+Proof.
+  split.
+  - intros; exists b.
+    apply ord_join in H.
+    apply join_comm; auto.
+  - intros (? & H); apply join_ord in H; tauto.
+Qed.
+
+(* The master-snapshot PCM in the RCU paper divides the master into shares, which is useful for having both
+   an authoritative writer and an up-to-date invariant. *)
+
+Global Program Instance snap_PCM : Ghost :=
+  { valid _ := True; Join_G a b c := sepalg.join (fst a) (fst b) (fst c) /\
+      if eq_dec (fst a) Share.bot then if eq_dec (fst b) Share.bot then join (snd a) (snd b) (snd c)
+        else ord (snd a) (snd b) /\ snd c = snd b else snd c = snd a /\
+          if eq_dec (fst b) Share.bot then ord (snd b) (snd a) else snd c = snd b }.
+Next Obligation.
+  exists (fun '(sh, a) => (Share.bot, core a)); repeat intro.
+  + destruct t; constructor; auto; simpl.
+    rewrite eq_dec_refl.
+    if_tac; [apply core_unit | split; auto].
+    rewrite join_ord_eq; eexists; apply core_unit.
+  + destruct a, b, c; f_equal.
+    inv H; simpl in *.
+    destruct (eq_dec t Share.bot); [|destruct H1; subst; auto].
+    subst; apply bot_identity in H0; subst.
+    destruct (eq_dec t1 Share.bot); [|destruct H1; subst; auto].
+    * eapply join_core; eauto.
+    * apply join_ord_eq in H; destruct H.
+      eapply join_core; eauto.
+Defined.
+Next Obligation.
+  constructor.
+  - intros ???? [? Hjoin1] [? Hjoin2].
+    assert (fst z = fst z') by (eapply join_eq; eauto).
+    destruct z, z'; simpl in *; subst; f_equal.
+    destruct (eq_dec (fst x) Share.bot); [|destruct Hjoin1, Hjoin2; subst; auto].
+    destruct (eq_dec (fst y) Share.bot); [|destruct Hjoin1, Hjoin2; subst; auto].
+    eapply join_eq; eauto.
+  - intros ????? [Hsh1 Hjoin1] [Hsh2 Hjoin2].
+    destruct (sepalg.join_assoc Hsh1 Hsh2) as [sh' []].
+    destruct (eq_dec (fst b) Share.bot) eqn: Hb.
+    + assert (fst d = fst a) as Hd.
+      { eapply sepalg.join_eq; eauto.
+        rewrite e0; apply join_bot_eq. }
+      rewrite Hd in Hsh1, Hsh2, Hjoin2.
+      assert (sh' = fst c) as Hc.
+      { eapply sepalg.join_eq; eauto.
+        rewrite e0; apply bot_join_eq. }
+      subst sh'.
+      destruct (eq_dec (fst c) Share.bot) eqn: Hc1.
+      * destruct (eq_dec (fst a) Share.bot) eqn: Ha.
+        -- destruct (join_assoc Hjoin1 Hjoin2) as [c' []].
+            destruct a, b, c; simpl in *; subst.
+           exists (Share.bot, c'); split; split; rewrite ?eq_dec_refl; auto.
+        -- destruct Hjoin1 as [Hc' ?]; rewrite Hc' in Hjoin2.
+           destruct Hjoin2, (ord_lub (snd b) (snd c) (snd a)) as [c' []]; eauto.
+           destruct b, c; simpl in *; subst.
+           exists (Share.bot, c'); split; split; rewrite ?eq_dec_refl, ?Ha; auto.
+      * exists c.
+        destruct (eq_dec (fst a) Share.bot) eqn: Ha; try solve [split; split; auto].
+        -- destruct Hjoin2.
+           apply join_ord in Hjoin1; destruct Hjoin1.
+           destruct b; simpl in *; subst.
+           split; split; rewrite ?Ha, ?Hc1, ?eq_dec_refl; auto; split; auto; etransitivity; eauto.
+        -- destruct Hjoin2 as [He1 He2].
+           destruct Hjoin1 as [Hd' ?]; rewrite He2, Hd' in He1; split; split; rewrite ?e0, ?He2, ?He1, ?Ha, ?Hc1, ?eq_dec_refl, ?Hd'; auto.
+    + exists (sh', snd b); simpl.
+      destruct (eq_dec (fst d) Share.bot).
+      { rewrite e0 in Hsh1; apply join_Bot in Hsh1; destruct Hsh1; contradiction. }
+      destruct (eq_dec sh' Share.bot) eqn: Hn'.
+      { subst; apply join_Bot in H; destruct H; contradiction. }
+      assert (snd d = snd b) as Hd by (destruct (eq_dec (fst a) Share.bot); tauto).
+      rewrite Hd in Hjoin1, Hjoin2; destruct Hjoin2 as [He Hjoin2]; rewrite He in Hjoin2; split; split; simpl; rewrite ?Hb, ?Hn', ?Hd, ?He; auto.
+  - intros ??? []; split; [apply join_comm; auto|].
+    if_tac; if_tac; auto; tauto.
+  - intros ???? [? Hjoin1] [? Hjoin2].
+    assert (fst a = fst b) by (eapply join_positivity; eauto).
+    destruct (eq_dec (fst a) Share.bot), a, a', b, b'; simpl in *; subst; f_equal.
+    + rewrite eq_dec_refl in Hjoin2.
+      apply join_Bot in H0 as []; subst.
+      apply join_Bot in H as []; subst.
+      rewrite !eq_dec_refl in Hjoin1, Hjoin2.
+      eapply join_positivity; eauto.
+    + destruct Hjoin1; auto.
+Defined.
+Next Obligation.
+  auto.
+Defined.
+
+Definition ghost_snap (a : @G P) p := own p (Share.bot, a) NoneP.
+
+Lemma ghost_snap_join : forall v1 v2 p v, join v1 v2 v ->
+  (ghost_snap v1 p * ghost_snap v2 p = ghost_snap v p)%pred.
+Proof.
+  intros; symmetry; apply ghost_op.
+  split; simpl; rewrite ?eq_dec_refl; auto.
+Qed.
+
+Lemma prop_derives : forall (P Q : Prop), (P -> Q) -> !!P |-- !!Q.
+Proof.
+  repeat intro; simpl in *; auto.
+Qed.
+
+Lemma ghost_snap_conflict : forall v1 v2 p, ghost_snap v1 p * ghost_snap v2 p |-- !!(joins v1 v2).
+Proof.
+  intros; eapply derives_trans; [apply ghost_valid_2|].
+  apply prop_derives.
+  intros ((?, a) & (? & Hj) & _); simpl in Hj.
+  rewrite !eq_dec_refl in Hj.
+  exists a; auto.
+Qed.
+
+Lemma ghost_snap_join' : forall v1 v2 p,
+  (ghost_snap v1 p * ghost_snap v2 p = EX v : _, !!(join v1 v2 v) && ghost_snap v p)%pred.
+Proof.
+  intros; apply pred_ext.
+  - eapply derives_trans, prop_andp_left; [apply andp_right, derives_refl; apply ghost_snap_conflict|].
+    intros [v]; apply exp_right with v; apply prop_andp_right; auto.
+    erewrite ghost_snap_join; eauto.
+  - apply exp_left; intro v; apply prop_andp_left; intro.
+    erewrite ghost_snap_join; eauto.
+Qed.
+
+Definition ghost_master sh (a : @G P) p := own p (sh, a) NoneP.
+
+Lemma snap_master_join : forall v1 sh v2 p, sh <> Share.bot ->
+  (ghost_snap v1 p * ghost_master sh v2 p = !!(ord v1 v2) && ghost_master sh v2 p)%pred.
+Proof.
+  intros; setoid_rewrite own_op'.
+  apply pred_ext.
+  - apply exp_left; intro a3; apply prop_andp_left.
+    destruct a3 as (sh', ?); intros ([Hsh Hj] & _); simpl in *.
+    apply bot_identity in Hsh; subst sh'.
+    rewrite eq_dec_refl in Hj.
+    destruct (eq_dec sh Share.bot); [contradiction|].
+    destruct Hj; subst; apply prop_andp_right; auto.
+  - apply prop_andp_left; intro.
+    apply exp_right with (sh, v2), prop_andp_right; auto.
+    split; simpl; auto.
+    split; simpl; rewrite ?eq_dec_refl.
+    + apply bot_join_eq.
+    + if_tac; auto; contradiction.
+Qed.
+
+Corollary snaps_master_join : forall lv sh v2 p, sh <> Share.bot ->
+  (fold_right sepcon emp (map (fun v => ghost_snap v p) lv) * ghost_master sh v2 p =
+  !!(Forall (fun v1 => ord v1 v2) lv) && ghost_master sh v2 p)%pred.
+Proof.
+  induction lv; simpl; intros.
+  - rewrite emp_sepcon, prop_true_andp; auto.
+  - rewrite sepcon_comm, <-sepcon_assoc, (sepcon_comm (ghost_master _ _ _)), snap_master_join; auto.
+    apply pred_ext.
+    + rewrite sepcon_andp_prop1; apply prop_andp_left; intro.
+      rewrite sepcon_comm, IHlv by auto.
+      apply prop_andp_left; intro; apply prop_andp_right; auto.
+    + apply prop_andp_left; intros Hall.
+      inv Hall.
+      rewrite prop_true_andp; auto.
+      rewrite sepcon_comm, IHlv by auto.
+      apply prop_andp_right; auto.
+Qed.
+
+Lemma join_Tsh : forall a b, sepalg.join Tsh a b -> b = Tsh /\ a = Share.bot.
+Proof.
+  intros ?? (? & ?).
+  rewrite Share.glb_commute, Share.glb_top in H; subst; split; auto.
+  apply Share.lub_bot.
+Qed.
+
+Lemma master_update : forall v v' p, ord v v' -> ghost_master Tsh v p |-- |==> ghost_master Tsh v' p.
+Proof.
+  intros; apply ghost_update.
+  intros ? (x & Hj & _); simpl in Hj.
+  exists (Tsh, v'); simpl; split; auto.
+  destruct Hj as [Hsh Hj]; simpl in *.
+SearchAbout join Tsh.
+  apply join_Tsh in Hsh as []; destruct c, x; simpl in *; subst.
+  split; auto; simpl.
+  fold share in *; destruct (eq_dec Tsh Share.bot); [contradiction Share.nontrivial|].
+  destruct Hj as [? Hc']; subst.
+  rewrite !eq_dec_refl in Hc' |- *; split; auto.
+  etransitivity; eauto.
+Qed.
+
+Lemma master_init : forall (a : @G P), exists g', joins (Tsh, a) g'.
+Proof.
+  intros; exists (Share.bot, a), (Tsh, a); simpl.
+  split; auto; simpl.
+  apply join_refl.
+Qed.
+
+Hint Resolve bupd_intro : ghost.
+
+Lemma make_snap : forall (sh : share) v p, ghost_master sh v p |-- |==> ghost_snap v p * ghost_master sh v p.
+Proof.
+  intros.
+  destruct (eq_dec sh Share.bot).
+  - subst; setoid_rewrite ghost_snap_join; [|apply join_refl]; auto with ghost.
+  - rewrite snap_master_join by auto.
+    rewrite prop_true_andp by reflexivity; apply bupd_intro.
+Qed.
+
+Lemma ghost_snap_forget : forall v1 v2 p, ord v1 v2 -> ghost_snap v2 p |-- |==> ghost_snap v1 p.
+Proof.
+  intros; apply ghost_update.
+  intros (shc, c) [(shx, x) [[? Hj] _]]; simpl in *.
+  rewrite eq_dec_refl in Hj.
+  assert (shx = shc) by (eapply sepalg.join_eq; eauto); subst.
+  unfold share in Hj; destruct (eq_dec shc Share.bot); subst.
+  - destruct (join_compat _ _ _ _ Hj H) as [x' []].
+    exists (Share.bot, x'); simpl; split; auto; split; auto; simpl.
+    rewrite !eq_dec_refl; auto.
+  - destruct Hj; subst.
+    exists (shc, c); simpl; split; auto; split; auto; simpl.
+    rewrite eq_dec_refl; if_tac; [contradiction|].
+    split; auto.
+    etransitivity; eauto.
+Qed.
+
+Lemma ghost_snap_choose : forall v1 v2 p, ghost_snap v1 p * ghost_snap v2 p |-- |==> ghost_snap v1 p.
+Proof.
+  intros.
+  setoid_rewrite own_op'.
+  apply exp_left; intro v'; apply prop_andp_left; intros [H ?].
+  destruct v', H as [Hsh Hj]; apply bot_identity in Hsh; simpl in *; subst.
+  rewrite !eq_dec_refl in Hj.
+  apply ghost_snap_forget.
+  rewrite join_ord_eq; eauto.
+Qed.
+
+Lemma master_share_join : forall sh1 sh2 sh v p, sepalg.join sh1 sh2 sh ->
+  (ghost_master sh1 v p * ghost_master sh2 v p = ghost_master sh v p)%pred.
+Proof.
+  intros; symmetry; apply ghost_op; split; auto; simpl.
+  if_tac; if_tac; try split; auto; try reflexivity; apply join_refl.
+Qed.
+
+Lemma unreadable_bot : ~readable_share Share.bot.
+Proof.
+  unfold readable_share, nonempty_share, sepalg.nonidentity.
+  rewrite Share.glb_bot; auto.
+Qed.
+
+Lemma master_inj : forall sh1 sh2 v1 v2 p, readable_share sh1 -> readable_share sh2 ->
+  ghost_master sh1 v1 p * ghost_master sh2 v2 p |-- !!(v1 = v2).
+Proof.
+  intros.
+  eapply derives_trans; [apply ghost_valid_2|].
+  apply prop_derives; intros ((?, ?) & [[? Hj] _]); simpl in Hj.
+  fold share in *.
+  destruct (eq_dec sh1 Share.bot); [subst; contradiction unreadable_bot|].
+  destruct (eq_dec sh2 Share.bot); [subst; contradiction unreadable_bot|].
+  destruct Hj; subst; auto.
+Qed.
+
+Lemma master_share_join' : forall sh1 sh2 sh v1 v2 p, readable_share sh1 -> readable_share sh2 ->
+  sepalg.join sh1 sh2 sh ->
+  (ghost_master sh1 v1 p * ghost_master sh2 v2 p = !!(v1 = v2) && ghost_master sh v2 p)%pred.
+Proof.
+  intros; apply pred_ext.
+  - eapply derives_trans; [apply andp_right, derives_refl; apply master_inj; auto|].
+    apply prop_andp_left; intros; subst.
+    apply prop_andp_right; auto.
+    erewrite master_share_join; eauto.
+  - apply prop_andp_left; intro; subst.
+    erewrite master_share_join; eauto.
+Qed.
+
+(* useful when we only want to deal with full masters *)
+Definition ghost_master1 a p := ghost_master Tsh a p.
+
+Lemma snap_master_join1 : forall v1 v2 p,
+  (ghost_snap v1 p * ghost_master1 v2 p = !!(ord v1 v2) && ghost_master1 v2 p)%pred.
+Proof.
+  intros; apply snap_master_join, Share.nontrivial.
+Qed.
+
+Lemma snap_master_update1 : forall v1 v2 p v', ord v2 v' ->
+  ghost_snap v1 p * ghost_master1 v2 p |-- |==> ghost_snap v' p * ghost_master1 v' p.
+Proof.
+  intros; rewrite !snap_master_join1.
+  apply prop_andp_left; intro.
+  rewrite prop_true_andp by reflexivity.
+  apply master_update; auto.
+Qed.
+
+End Snapshot.
+
+Section Discrete.
+
+Program Instance discrete_PCM (A : Type) : Ghost := { valid a := True;
+  Join_G := Join_equiv A }.
+Next Obligation.
+  auto.
+Defined.
+
+Context {A : Type}.
+
+Global Instance discrete_order : PCM_order(P := discrete_PCM A) eq.
+Proof.
+  constructor; intros.
+  - typeclasses eauto.
+  - exists c; subst; split; hnf; auto.
+  - inv H; auto.
+  - subst; hnf; auto.
+Defined.
+
+End Discrete.
