veric/invariants.v
@@ -1,0 +1,1190 @@
+Require Import VST.msl.ghost.
+Require Import VST.msl.ghost_seplog.
+Require Import VST.msl.sepalg_generators.
+Require Import VST.msl.sepalg.
+Require Import VST.veric.seplog.
+Require Import VST.veric.compcert_rmaps.
+Require Import VST.veric.own.
+Require Import VST.veric.mpred.
+Require Import VST.veric.ghosts.
+Require Import VST.floyd.sublist.
+Import List ListNotations.
+
+Lemma cored_dup_cored : forall P, P && cored |-- ((P && cored) * (P && cored)) && cored.
+Proof.
+  intros; apply andp_right.
+  - apply cored_dup.
+  - apply andp_left2; auto.
+Qed.
+
+Lemma cored_sepcon: forall P Q, (P && cored) * (Q && cored) |-- (P * Q) && cored.
+Proof.
+  intros.
+  apply andp_right.
+  + apply sepcon_derives; apply andp_left1; auto.
+  + eapply derives_trans; [apply sepcon_derives; apply andp_left2, derives_refl|].
+      rewrite <- cored_duplicable; auto.
+Qed.
+
+Lemma cored_dup_gen : forall P, P |-- cored -> P |-- P * P.
+Proof.
+  intros.
+  erewrite (log_normalize.add_andp P) by apply H; apply cored_dup.
+Qed.
+
+Section Invariants.
+
+Program Instance unit_PCM : Ghost := { valid a := True; Join_G a b c := True }.
+
+Definition pred_of (P : mpred) := SomeP rmaps.Mpred (fun _ => P).
+
+Definition agree g (P : mpred) := own(RA := unit_PCM) g tt (pred_of P).
+
+Lemma agree_dup : forall g P, (agree g P = agree g P * agree g P)%pred.
+Proof.
+  intros; apply ghost_op; constructor.
+Qed.
+
+Lemma agree_join : forall g P1 P2, agree g P1 * agree g P2 |-- (|> P1 -* |> P2) * agree g P1.
+Proof.
+  intros.
+  intros ? (? & ? & ? & H1 & H2).
+  do 3 eexists; [apply core_unit|].
+  pose proof (ghost_of_join _ _ _ H) as J.
+  change (agree g P1) with (own.own(RA := unit_PCM) g tt (pred_of P1)) in H1.
+  destruct H1 as (? & Hid & H1).
+  change (agree g P2) with (own.own(RA := unit_PCM) g tt (pred_of P2)) in H2.
+  destruct H2 as (? & ? & H2).
+  erewrite H1, H2, !own.ghost_fmap_singleton in J.
+  apply own.singleton_join_inv in J as ([] & J & Jg).
+  inv J; simpl in *.
+  inv H4.
+  apply SomeP_inj in H5.
+  destruct (join_level _ _ _ H) as [Hl1 Hl2]; erewrite Hl1, Hl2 in *.
+  assert (approx (level a) P1 = approx (level a) P2) as Heq.
+  { apply (@equal_f _ _ (fun _ : list Type => approx (level a) P1) (fun _ : list Type => approx (level a) P2));
+      auto.
+    apply nil. }
+  split.
+  - intros ??? Hl J HP1 ? Ha'.
+    pose proof (level_core a).
+    pose proof (necR_level _ _ Hl).
+    apply nec_identity in Hl; [|apply core_identity].
+    destruct (join_level _ _ _ J).
+    apply Hl in J; subst.
+    specialize (HP1 _ Ha').
+    apply laterR_level in Ha'.
+    assert ((approx (level a) P1) a') as HP1'.
+    { split; auto; omega. }
+    rewrite Heq in HP1'; destruct HP1'; auto.
+  - exists I; split.
+    + intro l; simpl.
+      apply (resource_at_join _ _ _ l) in H.
+      apply Hid in H as <-; auto.
+    + simpl; erewrite Jg, own.ghost_fmap_singleton; simpl.
+      repeat f_equal; auto.
+      inv H3; f_equal.
+      destruct c0; apply exist_ext; auto.
+Qed.
+
+Lemma agree_join2 : forall g P1 P2, agree g P1 * agree g P2 |-- (|> P1 -* |> P2) * agree g P2.
+Proof.
+  intros.
+  intros ? (? & ? & ? & H1 & H2).
+  do 3 eexists; [apply core_unit|].
+  pose proof (ghost_of_join _ _ _ H) as J.
+  change (agree g P1) with (own.own(RA := unit_PCM) g tt (pred_of P1)) in H1.
+  destruct H1 as (? & Hid & H1).
+  change (agree g P2) with (own.own(RA := unit_PCM) g tt (pred_of P2)) in H2.
+  destruct H2 as (? & ? & H2).
+  erewrite H1, H2, !own.ghost_fmap_singleton in J.
+  apply own.singleton_join_inv in J as ([] & J & Jg).
+  inv J; simpl in *.
+  inv H4.
+  apply SomeP_inj in H5.
+  destruct (join_level _ _ _ H) as [Hl1 Hl2]; erewrite Hl1, Hl2 in *.
+  assert (approx (level a) P1 = approx (level a) P2) as Heq.
+  { apply (@equal_f _ _ (fun _ : list Type => approx (level a) P1) (fun _ : list Type => approx (level a) P2));
+      auto.
+    apply nil. }
+  split.
+  - intros ??? Hl J HP1 ? Ha'.
+    pose proof (level_core a).
+    pose proof (necR_level _ _ Hl).
+    apply nec_identity in Hl; [|apply core_identity].
+    destruct (join_level _ _ _ J).
+    apply Hl in J; subst.
+    specialize (HP1 _ Ha').
+    apply laterR_level in Ha'.
+    assert ((approx (level a) P1) a') as HP1'.
+    { split; auto; omega. }
+    rewrite Heq in HP1'; destruct HP1'; auto.
+  - exists I; split.
+    + intro l; simpl.
+      apply (resource_at_join _ _ _ l) in H.
+      apply Hid in H as <-; auto.
+    + simpl; erewrite Jg, own.ghost_fmap_singleton; simpl.
+      repeat f_equal; auto.
+      inv H3; f_equal.
+      destruct c0; apply exist_ext; auto.
+Qed.
+
+Inductive list_join {P : Ghost} : Join (list (option G)) :=
+  | list_join_nil_l m: list_join nil m m
+  | list_join_nil_r m: list_join m nil m
+  | list_join_cons a1 a2 m1 m2 a3 m3: join a1 a2 a3 -> list_join m1 m2 m3 ->
+      list_join (a1 :: m1) (a2 :: m2) (a3 :: m3).
+Existing Instance list_join.
+
+Lemma list_join_inv: forall {P : Ghost} (l1 l2 l3 : list (option G)), list_join l1 l2 l3 ->
+match l1, l2 with
+| nil, _ => l3 = l2
+| _, nil => l3 = l1
+| a1 :: l1, a2 :: l2 => match l3 with nil => False
+                        | a3 :: l3 => join a1 a2 a3 /\ list_join l1 l2 l3 end
+end.
+Proof.
+  induction 1; simpl; auto.
+  destruct m; simpl; auto.
+Qed.
+
+Program Instance list_PCM (P : Ghost) : Ghost := { valid a := True; Join_G := list_join(*; core2 := map core2*) }.
+Next Obligation.
+Proof.
+  intros; exists (fun _ => nil); auto; constructor.
+Defined.
+Next Obligation.
+  constructor.
+    + intros until 1.
+      revert z'; induction H; inversion 1; auto; subst.
+      f_equal; eauto.
+      eapply join_eq; eauto.
+    + induction a; intros ???? J1 J2; eapply list_join_inv in J1; subst.
+      { exists e; split; auto; constructor. }
+      destruct b; subst; [eexists; split; eauto; constructor|].
+      destruct d; [contradiction|].
+      destruct J1 as [Jc1 J1].
+      apply list_join_inv in J2.
+      destruct c; subst; [eexists; split; eauto; constructor; auto|].
+      destruct e; [contradiction|].
+      destruct J2 as [Jc2 J2].
+      destruct (join_assoc Jc1 Jc2) as (f & ? & ?).
+      destruct (IHa _ _ _ _ J1 J2) as (f' & ? & ?).
+      exists (f :: f'); split; constructor; auto.
+    + induction 1; constructor; auto.
+    + intros until 1.
+      revert b'; induction H; inversion 1; auto; subst.
+      f_equal; eauto.
+      eapply join_positivity; eauto.
+Qed.
+
+Definition ghost_list {P : Ghost} g l := own(RA := list_PCM P) g l NoneP.
+
+Definition list_singleton {A} n (a : A) := repeat None n ++ [Some a].
+
+Definition list_incl {A} (l1 l2 : list (option A)) := (length l1 <= length l2)%nat /\
+  forall n a, nth n l1 None = Some a -> nth n l2 None = Some a.
+
+(* up *)
+Lemma app_nth : forall {A} n l1 l2 (d : A),
+  nth n (l1 ++ l2) d = if lt_dec n (length l1) then nth n l1 d else nth (n - length l1) l2 d.
+Proof.
+  intros.
+  if_tac; [rewrite app_nth1 | rewrite app_nth2]; auto; omega.
+Qed.
+
+Fixpoint replace_nth {A} (n: nat) (al: list A) (x: A) {struct n}: list A :=
+ match n, al with
+ | O , a::al => x::al
+ | S n', a::al' => a :: replace_nth n' al' x
+ | _, nil => nil
+ end.
+
+Lemma replace_nth_length : forall {A} n l (a : A),
+  length (replace_nth n l a) = length l.
+Proof.
+  induction n; destruct l; simpl; intros; try omega.
+  erewrite IHn by omega; auto.
+Qed.
+
+Lemma replace_nth_app : forall {A} n l1 l2 (a : A),
+  replace_nth n (l1 ++ l2) a = if lt_dec n (length l1) then replace_nth n l1 a ++ l2
+  else l1 ++ replace_nth (n - length l1) l2 a.
+Proof.
+  induction n; destruct l1; auto; simpl; intros.
+  rewrite IHn.
+  if_tac; if_tac; auto; omega.
+Qed.
+
+Lemma list_join_app : forall {P : Ghost} l1 l2 m1 m2 n1 n2,
+  length l1 = length m1 -> length l1 = length n1 ->
+  list_join l1 m1 n1 -> list_join l2 m2 n2 ->
+  list_join (l1 ++ l2) (m1 ++ m2) (n1 ++ n2).
+Proof.
+  induction 3.
+  - destruct m; auto; discriminate.
+  - destruct m; auto; discriminate.
+  - simpl in *.
+    intros; constructor; auto.
+Qed.
+
+Lemma list_join_None : forall {P : Ghost} n l, (n <= length l)%nat ->
+  list_join (repeat None n) l l.
+Proof.
+  induction n; [constructor|].
+  destruct l; simpl; [omega|].
+  repeat constructor.
+  apply IHn; omega.
+Qed.
+
+Lemma list_join_over : forall {P : Ghost} l l1 l2 l1', (length l <= length l1)%nat ->
+  list_join l l1 l1' -> list_join l (l1 ++ l2) (l1' ++ l2).
+Proof.
+  induction 2; simpl in *.
+  - constructor.
+  - destruct m; [constructor | simpl in *; omega].
+  - constructor; auto.
+    apply IHlist_join; omega.
+Qed.
+
+Lemma singleton_length : forall {A} n (a : A), length (list_singleton n a) = S n.
+Proof.
+  intros; unfold list_singleton.
+  erewrite app_length, repeat_length; simpl; omega.
+Qed.
+
+Lemma list_join_singleton : forall {P : Ghost} n a c l
+  (Hn : (n < length l)%nat) (Hjoin: join (Some a) (nth n l None) (Some c)),
+  list_join (list_singleton n a) l (replace_nth n l (Some c)).
+Proof.
+  induction l using rev_ind; simpl; intros; try omega.
+  rewrite app_length in Hn; simpl in Hn.
+  destruct (eq_dec n (length l)).
+  - subst.
+    erewrite app_nth2, minus_diag in Hjoin by omega; simpl in Hjoin.
+    erewrite replace_nth_app, if_false, minus_diag by omega; simpl.
+    apply list_join_app; try (rewrite repeat_length; auto).
+    + apply list_join_None; auto.
+    + repeat constructor; auto.
+  - assert (n < length l)%nat by omega.
+    erewrite app_nth1 in Hjoin by auto.
+    erewrite replace_nth_app, if_true by auto.
+    apply list_join_over, IHl; auto.
+    rewrite singleton_length; omega.
+Qed.
+
+(* up *)
+Lemma replace_nth_same : forall {A} n l (d : A), replace_nth n l (nth n l d) = l.
+Proof.
+  induction n; destruct l; auto; simpl; intro.
+  rewrite IHn; auto.
+Qed.
+
+Lemma nth_replace_nth : forall {A} n l a (d : A), (n < length l)%nat ->
+  nth n (replace_nth n l a) d = a.
+Proof.
+  induction n; destruct l; auto; simpl; intros; try omega.
+  apply IHn; omega.
+Qed.
+
+Lemma nth_replace_nth' : forall {A} n m l a (d : A), m <> n ->
+  nth m (replace_nth n l a) d = nth m l d.
+Proof.
+  induction n; destruct l; auto; destruct m; auto; simpl; intros; try omega.
+  apply IHn; omega.
+Qed.
+
+Lemma Znth_replace_nth : forall {A} {d : Inhabitant A} n l (a : A), (n < length l)%nat ->
+  Znth (Z.of_nat n) (replace_nth n l a) = a.
+Proof.
+  intros; rewrite <- nth_Znth'.
+  apply nth_replace_nth; auto.
+Qed.
+
+Lemma Znth_replace_nth' : forall {A} {d : Inhabitant A} n m l (a : A), m <> Z.of_nat n ->
+  Znth m (replace_nth n l a) = Znth m l.
+Proof.
+  intros.
+  destruct (zlt m 0); [rewrite !Znth_underflow; auto|].
+  rewrite <- (Z2Nat.id m) by omega.
+  rewrite <- !nth_Znth'; apply nth_replace_nth'.
+  intro; contradiction H; subst.
+  erewrite Z2Nat.id by omega; auto.
+Qed.
+
+Lemma replace_nth_replace_nth: forall {A: Type} R n {Rn Rn': A},
+  replace_nth n (replace_nth n R Rn) Rn' = replace_nth n R Rn'.
+Proof.
+  intros.
+  revert R; induction n; destruct R; simpl in *.
+  + reflexivity.
+  + reflexivity.
+  + reflexivity.
+  + rewrite IHn.
+    reflexivity.
+Qed.
+
+Lemma ghost_list_nth : forall {P : Ghost} g n l (a : G) (Ha : nth n l None = Some a),
+  (ghost_list g l = ghost_list g (list_singleton n a) * ghost_list g (replace_nth n l None))%pred.
+Proof.
+  intros; apply ghost_op.
+  rewrite <- (replace_nth_same n l None) at 2.
+  destruct (lt_dec n (length l)); [|erewrite nth_overflow in Ha by omega; discriminate].
+  exploit (list_join_singleton n a a (replace_nth n l None)).
+  { rewrite replace_nth_length; auto. }
+  { erewrite nth_replace_nth by auto; constructor. }
+  erewrite replace_nth_replace_nth, Ha; auto.
+Qed.
+
+Lemma list_join_length : forall {P : Ghost} l1 l2 l3, list_join l1 l2 l3 ->
+  (length l1 <= length l3)%nat.
+Proof.
+  induction 1; auto; simpl; omega.
+Qed.
+
+Lemma list_join_filler : forall {P : Ghost} l1 l2 l3 n, list_join l1 l2 l3 ->
+  (n <= length l3 - length l1)%nat -> list_join (l1 ++ repeat None n) l2 l3.
+Proof.
+  induction 1; simpl; intros.
+  - apply list_join_None; omega.
+  - destruct n; [|omega].
+    rewrite app_nil_r; constructor.
+  - constructor; auto.
+Qed.
+
+Lemma list_join_nth : forall {P : Ghost} l1 l2 l3 n, list_join l1 l2 l3 ->
+  join (nth n l1 None) (nth n l2 None) (nth n l3 None).
+Proof.
+  intros; revert n.
+  induction H; intro.
+  - erewrite nth_overflow by (simpl; omega); constructor.
+  - erewrite (nth_overflow []) by (simpl; omega); constructor.
+  - destruct n; simpl; auto.
+Qed.
+
+Lemma list_join_max : forall {P : Ghost} l1 l2 l3, list_join l1 l2 l3 ->
+  length l3 = Max.max (length l1) (length l2).
+Proof.
+  induction 1; simpl; auto.
+  rewrite Nat.max_l; auto; omega.
+Qed.
+
+Lemma list_join_nth_error : forall {P : Ghost} l1 l2 l3 n, list_join l1 l2 l3 ->
+  join (nth_error l1 n) (nth_error l2 n) (nth_error l3 n).
+Proof.
+  intros; revert n.
+  induction H; intro.
+  - rewrite nth_error_nil; constructor.
+  - rewrite nth_error_nil; constructor.
+  - destruct n; simpl; auto.
+    constructor; auto.
+Qed.
+
+Lemma list_join_alt : forall {P : Ghost} l1 l2 l3,
+  list_join l1 l2 l3 <-> forall n, join (nth_error l1 n) (nth_error l2 n) (nth_error l3 n).
+Proof.
+  split; [intros; apply list_join_nth_error; auto|].
+  revert l2 l3; induction l1; simpl; intros.
+  - assert (l2 = l3); [|subst; constructor].
+    apply list_nth_error_eq; intro.
+    specialize (H j); rewrite nth_error_nil in H; inv H; auto.
+  - destruct l2.
+    + assert (a :: l1 = l3); [|subst; constructor].
+      apply list_nth_error_eq; intro.
+      specialize (H j); rewrite nth_error_nil in H; inv H; auto.
+    + destruct l3.
+      { specialize (H O); inv H. }
+      constructor.
+      * specialize (H O); inv H; auto.
+      * apply IHl1; intro.
+        apply (H (S n)).
+Qed.
+
+Lemma nth_error_replace_nth : forall {A} n l (a : A), (n < length l)%nat ->
+  nth_error (replace_nth n l a) n = Some a.
+Proof.
+  induction n; destruct l; auto; simpl; intros; try omega.
+  apply IHn; omega.
+Qed.
+
+Lemma nth_error_replace_nth' : forall {A} n m l (a : A), m <> n ->
+  nth_error (replace_nth n l a) m = nth_error l m.
+Proof.
+  induction n; destruct l; auto; destruct m; auto; simpl; intros; try omega.
+  apply IHn; omega.
+Qed.
+
+Instance list_order A : @PCM_order (list_PCM (discrete_PCM A)) list_incl.
+Proof.
+  constructor.
+  - constructor.
+    + repeat intro; split; auto.
+    + repeat intro.
+      destruct H, H0; split; auto; omega.
+  - intro a.
+    remember (length a) as n.
+    revert dependent a; induction n; intros.
+    + destruct a; inv Heqn.
+      exists b; split; auto.
+      change [] with (core b); apply core_unit.
+    + assert (a <> []) by (intro; subst; discriminate).
+      erewrite (app_removelast_last None) in H, Heqn by auto.
+      erewrite app_length in Heqn; simpl in Heqn.
+      erewrite Nat.add_1_r in Heqn; inv Heqn.
+      specialize (IHn _ eq_refl).
+      destruct (IHn b c) as (c' & ? & ?); auto.
+      { destruct H as [Hlen H].
+        split.
+        { rewrite app_length in Hlen; simpl in *; omega. }
+        intros ?? Hnth.
+        specialize (H n a0).
+        rewrite app_nth in H.
+        if_tac in H; auto.
+        rewrite nth_overflow in Hnth; [discriminate|].
+        apply not_lt; auto. }
+      pose proof (list_join_length _ _ _ H2).
+      pose proof (list_join_length _ _ _ (join_comm H2)).
+      destruct (eq_dec (length (removelast a)) (length c')).
+      * exists (c' ++ [List.last a None]); split.
+        -- erewrite (app_removelast_last None) at 1 by auto.
+           apply join_comm, list_join_over; try omega.
+           apply join_comm in H2; auto.
+        -- split.
+            { destruct H.
+              erewrite app_length in *; simpl in *; omega. }
+            intros ?? Hnth.
+            rewrite app_nth in Hnth.
+            if_tac in Hnth; [apply H3; auto|].
+            destruct (n - length c')%nat eqn: Hminus; [|destruct n0; discriminate].
+            simpl in Hnth.
+            apply H.
+            erewrite app_nth2 by omega.
+            replace (_ - _)%nat with O by omega; auto.
+       * destruct (List.last a None) eqn: Ha.
+         -- exists (replace_nth (length (removelast a)) c' (Some g)).
+            split.
+            ++ apply list_join_alt; intro.
+               pose proof (list_join_max _ _ _ H2) as Hlen.
+               destruct (Max.max_spec (length (removelast a)) (length b)) as [[? Hmax] | [? Hmax]];
+                 setoid_rewrite Hmax in Hlen; try omega.
+               hnf in H2; erewrite list_join_alt in H2.
+               specialize (H2 n0).
+               erewrite (app_removelast_last None) at 1 by auto.
+               rewrite Ha.
+               destruct (lt_dec n0 (length (removelast a))).
+               ** erewrite nth_error_app1 by auto.
+                  erewrite nth_error_replace_nth' by omega; auto.
+               ** erewrite nth_error_app2 by omega.
+                  destruct (eq_dec n0 (length (removelast a))).
+                  { subst; rewrite minus_diag; simpl.
+                    erewrite nth_error_replace_nth by (simpl in *; omega).
+                    destruct (nth_error b (length (removelast a))) eqn: Hb; setoid_rewrite Hb; constructor.
+                    destruct o; constructor.
+                    destruct H0 as [_ Hc].
+                    erewrite nth_error_nth in Hb by auto.
+                    inv Hb.
+                    apply Hc in H7.
+                    destruct H as [_ Hc'].
+                    specialize (Hc' (length (removelast a))).
+                    erewrite app_nth2, minus_diag in Hc' by auto.
+                    setoid_rewrite Hc' in H7; [|reflexivity].
+                    inv H7; constructor; auto. }
+                  { destruct (_ - _)%nat eqn: Hminus; [omega | simpl].
+                    erewrite nth_error_nil, nth_error_replace_nth' by (simpl in *; omega).
+                    destruct (nth_error_length n0 (removelast a)) as [_ Hnone].
+                    setoid_rewrite Hnone in H2; [auto | omega]. }
+            ++ destruct H3.
+               split.
+               { rewrite replace_nth_length; auto. }
+               intros ?? Hnth.
+               destruct (eq_dec n0 (length (removelast a)));
+                 [|rewrite nth_replace_nth' in Hnth; auto].
+               subst; erewrite nth_replace_nth in Hnth by (simpl in *; omega).
+               inv Hnth.
+               apply H.
+               erewrite app_nth2, minus_diag; auto.
+         -- exists c'; split; auto.
+            erewrite (app_removelast_last None), Ha by auto.
+            apply list_join_filler with (n0 := 1%nat); auto; simpl in *; omega.
+  - split.
+    + split; [eapply list_join_length; eauto|].
+      intros ?? Hnth.
+      apply list_join_nth with (n0 := n) in H.
+      rewrite Hnth in H; inv H; auto.
+      inv H3; auto.
+    + split; [apply join_comm in H; eapply list_join_length; eauto|].
+      intros ?? Hnth.
+      apply list_join_nth with (n0 := n) in H.
+      rewrite Hnth in H; inv H; auto.
+      inv H3; auto.
+  - induction a; unfold list_incl; intros.
+    + destruct b; [constructor|].
+      simpl in *; omega.
+    + destruct H as [? Hnth].
+      destruct b; constructor.
+      * destruct o; [|constructor].
+        specialize (Hnth O _ eq_refl); simpl in Hnth.
+        subst; repeat constructor.
+      * apply IHa.
+        split; [simpl in *; omega|].
+        intros.
+        apply (Hnth (S n)); auto.
+Qed.
+
+(*Notation union := base.union.
+
+Program Instance set_PCM : Ghost := { valid := fun _ : coPset => True;
+  Join_G a b c := a ## b /\ c = union a b(*; core2 a := empty*) }.
+Next Obligation.
+Proof.
+  exists (fun _ => empty); auto.
+  intro; split; set_solver.
+Defined.
+Next Obligation.
+  constructor.
+    + intros.
+      inv H; inv H0; auto.
+    + intros.
+      inv H; inv H0.
+      eexists; split; [split; eauto | split]; set_solver.
+    + intros.
+      inv H.
+      split; set_solver.
+    + intros.
+      inv H; inv H0.
+      set_solver.
+Qed.*)
+
+Import Ensembles.
+
+Program Instance set_PCM : Ghost := { valid := fun _ : Ensemble nat => True;
+  Join_G a b c := Disjoint _ a b /\ c = Union _ a b(*; core2 a := empty*) }.
+Next Obligation.
+Proof.
+  exists (fun _ => Empty_set _); auto.
+  intro; split.
+  - constructor; intros ? X.
+    inv X.
+    inv H.
+  - apply Extensionality_Ensembles; constructor; intros ??.
+    + right; auto.
+    + inv H; auto.
+      inv H0.
+Defined.
+Next Obligation.
+  constructor.
+    + intros ???? [] []; subst; auto.
+    + intros ????? [Hd1] [Hd2]; subst.
+      inv Hd1; inv Hd2.
+      exists (Union _ b c); repeat (split; auto).
+      * intros ? X; inv X.
+        contradiction (H0 x).
+        constructor; auto.
+        right; auto.
+      * intros ? X; inv X.
+        inv H2.
+        -- contradiction (H x); constructor; auto.
+        -- contradiction (H0 x); constructor; auto.
+           left; auto.
+      * apply Extensionality_Ensembles; constructor; intros ? X.
+        -- inv X; [|right; right; auto].
+           inv H1; [left | right; left]; auto.
+        -- inv X; [left; left; auto|].
+           inv H1; [left; right | right]; auto.
+    + intros ??? []; subst.
+      split.
+      * inv H; constructor.
+        intros x X; inv X; contradiction (H0 x); constructor; auto.
+      * apply Extensionality_Ensembles; constructor; intros ? X; inv X; first [(left; auto; fail) | (right; auto; fail)].
+    + intros ???? [] []; subst.
+      apply Extensionality_Ensembles; constructor; intros ? X.
+      { left; auto. }
+      rewrite H2; left; auto.
+Qed.
+
+Definition ghost_set g s := own(RA := set_PCM) g s NoneP.
+
+Lemma ghost_set_join : forall g s1 s2,
+  (ghost_set g s1 * ghost_set g s2 = !!(Disjoint _ s1 s2) && ghost_set g (Union _ s1 s2))%pred.
+Proof.
+  intros.
+  setoid_rewrite own_op_gen.
+  - instantiate (1 := Union _ s1 s2).
+    unfold ghost_set; apply pred_ext.
+    + apply prop_andp_left; intros (? & (? & []) & ?).
+      apply prop_andp_right; auto.
+    + apply prop_andp_left; intros.
+      apply prop_andp_right; auto.
+      eexists; repeat (split; auto).
+  - intros (? & H & ?); inv H; split; auto.
+Qed.
+
+Lemma ghost_set_subset : forall g s s' (Hdec : forall a, In _ s' a \/ ~In _ s' a),
+  (Included _ s' s -> ghost_set g s = ghost_set g s' * ghost_set g (Setminus _ s s'))%pred.
+Proof.
+  intros.
+  apply ghost_op.
+  split.
+  - constructor; intros ? X; inv X.
+    inv H1; contradiction.
+  - apply Extensionality_Ensembles; constructor; intros ? X.
+    + destruct (Hdec x); [left | right; constructor]; auto.
+    + inv X; auto.
+      inv H0; auto.
+Qed.
+
+Corollary ghost_set_remove : forall g a s,
+  In _ s a -> (ghost_set g s = ghost_set g (Singleton _ a) * ghost_set g (Subtract _ s a))%pred.
+Proof.
+  intros; apply ghost_set_subset.
+  { intro b; destruct (eq_dec a b); [left; subst; constructor | right; intros X; inv X; contradiction]. }
+  intros ? X; inv X; auto.
+Qed.
+
+Definition iname := nat.
+
+Class invG := { g_inv : gname; g_en : gname; g_dis : gname }.
+
+Context {inv_names : invG}.
+
+Definition master_list {A} g (l : list (option A)) := ghost_master1(ORD := list_order A) l g.
+
+(* Our ghost state construction makes it awkward to put agree inside other ghost state constructions.
+   As a workaround, instead of having one ghost location with a map from indices to agrees,
+   we have a map from indices to ghost locations, each with an agree. *)
+
+Instance token_PCM : Ghost := exclusive_PCM unit.
+
+Fixpoint iter_sepcon {A} (p : A -> mpred) l :=
+  match l with
+    | nil => emp
+    | x :: xl => (p x * iter_sepcon p xl)%pred
+  end.
+
+Typeclasses eauto := 1.
+
+Instance Inhabitant_mpred : Inhabitant mpred := emp.
+
+Definition wsat : mpred := (EX I : list mpred, EX lg : list gname, EX lb : list (option bool),
+  !!(length lg = length I /\ length lb = length I) &&
+  master_list g_inv (map (fun i => match Znth i lb with Some _ => Some (Znth i lg)
+                                   | None => None end) (upto (length I))) *
+  ghost_list g_dis (map (fun o => match o with Some true => Some (Some tt) | _ => None end) lb) *
+  ghost_set g_en (fun i : iname => nth i lb None = Some false) *
+  iter_sepcon (fun i => match Znth i lb with
+                        | Some true => agree (Znth i lg) (Znth i I) * |> Znth i I
+                        | Some false => agree (Znth i lg) (Znth i I)
+                        | _ => emp end) (upto (length I)))%pred.
+
+(* This is what's called ownI in Iris; we could build another layer with namespaces. *)
+Definition invariant (i : iname) P : mpred := (EX g : gname,
+  ghost_snap(ORD := list_order _) (list_singleton i g) g_inv * agree g P)%pred.
+
+Lemma nth_singleton : forall {A} n (a : A) d, nth n (list_singleton n a) d = Some a.
+Proof.
+  intros; unfold list_singleton.
+  rewrite app_nth2; rewrite repeat_length; auto.
+  rewrite minus_diag; auto.
+Qed.
+
+Lemma list_join_singleton_inv : forall {P : Ghost} n a b l,
+  list_join (list_singleton n a) (list_singleton n b) l ->
+  exists c, join a b c /\ l = list_singleton n c.
+Proof.
+  induction n; inversion 1; subst.
+  - inv H5.
+    inv H6; eauto.
+  - edestruct IHn as (c & ? & ?); eauto; subst.
+    inv H5; eauto.
+Qed.
+
+Lemma singleton_join_self : forall {P: Ghost} k (a : G), join a a a ->
+  join (list_singleton k a) (list_singleton k a) (list_singleton k a).
+Proof.
+  intros.
+  induction k; repeat constructor; auto.
+Qed.
+
+(* not currently useful *)
+(*Global Instance invariant_persistent i P : Persistent (invariant i P).
+Proof.
+  apply bi.exist_persistent; intro.
+  apply bi.sep_persistent; apply own_persistent; hnf; simpl; auto.
+  rewrite !eq_dec_refl; split; auto.
+  apply @singleton_join_self, join_refl.
+Qed.*)
+
+Lemma invariant_cored : forall i P, invariant i P |-- cored.
+Proof.
+  intros; unfold invariant.
+  apply exp_left; intro g.
+  rewrite cored_duplicable.
+  apply sepcon_derives; apply own_cored; hnf; auto; simpl.
+  split; auto.
+  rewrite !eq_dec_refl.
+  apply (singleton_join_self(P := discrete_PCM _)).
+  constructor; auto.
+Qed.
+
+Lemma invariant_dup : forall i P, (invariant i P = invariant i P * invariant i P)%pred.
+Proof.
+  intros; unfold invariant; apply pred_ext.
+  - apply exp_left; intro g.
+    rewrite exp_sepcon1; apply exp_right with g.
+    rewrite exp_sepcon2; apply exp_right with g.
+    rewrite <- sepcon_assoc, (sepcon_comm _ (ghost_snap _ _)), <- sepcon_assoc.
+    erewrite ghost_snap_join.
+    erewrite sepcon_assoc, <- agree_dup; apply derives_refl.
+    { apply (singleton_join_self(P := discrete_PCM _)).
+      constructor; auto. }
+  - rewrite exp_sepcon1; apply exp_left; intro g1.
+    rewrite exp_sepcon2; apply exp_left; intro g2.
+    erewrite <- sepcon_assoc, (sepcon_comm _ (ghost_snap _ _)), <- sepcon_assoc.
+    rewrite ghost_snap_join'.
+    rewrite !exp_sepcon1; apply exp_left; intro l.
+    rewrite !sepcon_andp_prop1; apply prop_andp_left; intro H.
+    apply (list_join_singleton_inv(P := discrete_PCM _)) in H as (g & H & ?); subst.
+    inv H.
+    erewrite sepcon_assoc, <- agree_dup.
+    apply exp_right with g; apply derives_refl.
+Qed.
+
+(* up *)
+Lemma Zlength_eq : forall {A B} (l1 : list A) (l2 : list B),
+  Zlength l1 = Zlength l2 <-> length l1 = length l2.
+Proof.
+  intros; rewrite !Zlength_correct.
+  split; [apply Nat2Z.inj|].
+  intro; apply Z2Nat.inj; try omega.
+  rewrite !Nat2Z.id; auto.
+Qed.
+
+Instance list_Perm {P : Ghost} : Perm_alg (list (option G)).
+Proof.
+  apply list_PCM.
+Qed.
+
+(* up *)
+Lemma nth_upto : forall m n d, (n < m)%nat -> nth n (upto m) d = Z.of_nat n.
+Proof.
+  intros.
+  erewrite nth_indep by (rewrite upto_length; auto).
+  erewrite nth_Znth', Znth_upto; auto.
+  split; [omega|].
+  apply Nat2Z.inj_lt; auto.
+Qed.
+
+Lemma nth_repeat : forall {A} n m (a : A), nth n (repeat a m) a = a.
+Proof.
+  induction n; destruct m; simpl; auto.
+Qed.
+
+Lemma list_incl_singleton : forall {A} n (a : A) l,
+  list_incl (list_singleton n a) l <-> nth n l None = Some a.
+Proof.
+  unfold list_incl; split.
+  - intros [? Hnth].
+    apply Hnth.
+    rewrite nth_singleton; auto.
+  - intros; split.
+    + rewrite singleton_length.
+      destruct (lt_dec n (length l)); [omega|].
+      erewrite nth_overflow in H by omega; discriminate.
+    + intros ??.
+      unfold list_singleton.
+      destruct (lt_dec n0 n).
+      * erewrite app_nth1 by (rewrite repeat_length; auto).
+        rewrite nth_repeat; discriminate.
+      * rewrite app_nth2; rewrite repeat_length; try omega.
+        destruct (eq_dec n0 n); [|erewrite nth_overflow by (simpl; omega); discriminate].
+        subst; rewrite minus_diag; simpl.
+        intro X; inv X; auto.
+Qed.
+
+Lemma seq_app : forall a b c, seq a (b + c) = seq a b ++ seq (a + b) c.
+Proof.
+  intros ??; revert a; induction b; simpl; intros; auto.
+  rewrite IHb; do 3 f_equal; omega.
+Qed.
+
+Lemma filter_ext_in : forall {A} (f g : A -> bool) l, (forall x, List.In x l -> f x = g x) -> filter f l = filter g l.
+Proof.
+  induction l; auto; simpl; intros.
+  rewrite -> H by auto.
+  rewrite IHl; auto.
+Qed.
+
+Lemma filter_none : forall {A} (f : A -> bool) l, (forall x, List.In x l -> f x = false) -> filter f l = [].
+Proof.
+  induction l; auto; simpl; intros.
+  rewrite H; auto.
+Qed.
+
+Ltac view_shift H := eapply derives_trans; [apply sepcon_derives, derives_refl; apply H
+  | eapply derives_trans; [apply bupd_frame_r | eapply derives_trans, bupd_trans; apply bupd_mono]].
+
+Lemma iter_sepcon_app:
+  forall {B} p (l1 l2 : list B), (iter_sepcon p (l1 ++ l2) = iter_sepcon p l1 * iter_sepcon p l2)%pred.
+Proof.
+  induction l1; intros; simpl. rewrite emp_sepcon; auto. rewrite IHl1. rewrite sepcon_assoc. auto.
+Qed.
+
+Lemma iter_sepcon_func_strong: forall {A} (l : list A) P Q, (forall x, List.In x l -> P x = Q x) -> iter_sepcon P l = iter_sepcon Q l.
+Proof.
+  intros. induction l.
+  + reflexivity.
+  + simpl.
+    f_equal.
+    - apply H.
+      simpl; auto.
+    - apply IHl.
+      intros; apply H.
+      simpl; auto.
+Qed. 
+
+Lemma iter_sepcon_emp': forall {B} p (l : list B), (forall x, List.In x l -> p x = emp) -> iter_sepcon p l = emp.
+Proof.
+  induction l; intros; simpl; auto.
+  rewrite H, IHl, sepcon_emp; simpl; auto.
+  intros; apply H; simpl; auto.
+Qed.
+
+Lemma wsat_alloc : forall P, wsat * |> P |-- |==> wsat * EX i : _, invariant i P.
+Proof.
+  intros; unfold wsat.
+  rewrite !exp_sepcon1; apply exp_left; intro l.
+  rewrite !exp_sepcon1; apply exp_left; intro lg.
+  rewrite !exp_sepcon1; apply exp_left; intro lb.
+  rewrite !sepcon_andp_prop1; apply prop_andp_left; intros [].
+  eapply derives_trans with (emp * _)%pred; [rewrite emp_sepcon; apply derives_refl|].
+  view_shift (ghost_alloc(RA := unit_PCM) tt (pred_of P)); [simpl; auto|].
+  rewrite !exp_sepcon1; apply exp_left; intro g.
+  replace (own(RA := unit_PCM) g tt (pred_of P)) with (agree g P) by reflexivity.
+  rewrite agree_dup.
+  rewrite <- !sepcon_assoc, (sepcon_comm _ (ghost_list _ _)), !sepcon_assoc.
+  view_shift (ghost_update_ND(RA := list_PCM token_PCM) g_dis (map
+     (fun o => match o with Some true => Some (Some tt) | _ => None end) lb)
+     (fun l => exists i, l =
+      map (fun o => match o with Some true => Some (Some tt) | _ => None end)
+          ((lb ++ repeat None i) ++ [Some true]))).
+  { intros ? (? & ? & _).
+    exists (map (fun o => match o with Some true => Some (Some tt) | _ => None end)
+      ((lb ++ repeat None (length x - length lb)) ++ [Some true])).
+    split; [eauto|].
+    exists (x ++ [Some (Some tt)]); split; simpl; auto.
+    erewrite !map_app, own.map_repeat; simpl.
+    pose proof (list_join_length _ _ _ H1) as Hlen.
+    rewrite map_length in Hlen.
+    apply join_comm in H1.
+    pose proof (list_join_length _ _ _ H1) as Hlen'.
+    apply (join_comm(Perm_alg := list_Perm)), (list_join_over c).
+    { erewrite app_length, map_length, repeat_length, le_plus_minus_r; auto. }
+    apply (join_comm(Perm_alg := list_Perm)), (list_join_filler(P := token_PCM));
+      [|rewrite map_length; auto].
+    apply join_comm in H1; auto. }
+  rewrite exp_sepcon1; apply exp_left; intro.
+  rewrite !sepcon_andp_prop1; apply prop_andp_left; intros [i ?]; subst.
+  assert (Zlength lg = Zlength l) as Hlg by (apply Zlength_eq; auto).
+  assert (Zlength lb = Zlength l) as Hlb by (apply Zlength_eq; auto).
+  rewrite <- !sepcon_assoc, (sepcon_comm _ (master_list _ _)), !sepcon_assoc.
+  view_shift (master_update(ORD := list_order _) ((map (fun i0 : Z =>
+      match Znth i0 lb with Some _ => Some (Znth i0 lg) | None => None end) (upto (Datatypes.length l))))
+        (map (fun j => match Znth j ((lb ++ repeat None i) ++ [Some true]) with
+                       | Some _ => Some (Znth j ((lg ++ repeat O i) ++ [g]))
+                       | None => None
+                       end) (upto (length ((l ++ repeat emp i) ++ [P]))))).
+  { rewrite <- !app_assoc, app_length, upto_app, map_app.
+    split.
+    { erewrite app_length, !map_length; omega. }
+    intros ?? Hn.
+    erewrite app_nth, map_length.
+    if_tac; [|erewrite nth_overflow in Hn by (rewrite map_length; omega); discriminate].
+    erewrite nth_map' with (d' := 0) in * by auto.
+    erewrite upto_length in *.
+    assert (Z.of_nat n < Zlength l).
+    { rewrite Zlength_correct; apply Nat2Z.inj_lt; auto. }
+    erewrite nth_upto in * by auto.
+    erewrite !app_Znth1 by omega; auto. }
+  view_shift (make_snap(ORD := list_order gname)).
+  rewrite !sepcon_assoc.
+  view_shift (ghost_snap_forget(ORD := list_order _) (list_singleton (length lg + i) g)).
+  { apply list_incl_singleton.
+    erewrite app_length, upto_app, map_app, app_nth2; erewrite map_length, upto_length, app_length,
+      repeat_length; try omega.
+    replace (_ - _)%nat with O by omega; simpl.
+    rewrite Nat2Z.inj_add, Z.add_0_r.
+    rewrite !app_Znth2; erewrite !Zlength_app, !Zlength_repeat, <- Zlength_correct; try omega.
+    replace (_ - _) with 0 by omega; replace (_ - _) with 0 by omega; auto. }
+  eapply derives_trans, bupd_intro.
+  apply exp_right with ((l ++ repeat emp i) ++ [P]).
+  rewrite exp_sepcon1; apply exp_right with ((lg ++ repeat O i) ++ [g]).
+  rewrite exp_sepcon1; apply exp_right with ((lb ++ repeat None i) ++ [Some true]).
+  erewrite !(app_length (_ ++ _)); simpl.
+  erewrite prop_true_andp by (erewrite !app_length, !repeat_length; omega).
+  erewrite upto_app, iter_sepcon_app; simpl.
+  erewrite Z.add_0_r, <- Zlength_correct, !app_Znth2; erewrite !Zlength_app, !Zlength_repeat; try omega.
+  erewrite Hlg, Hlb, Zminus_diag, !Znth_0_cons.
+  rewrite sepcon_comm, !sepcon_assoc; apply sepcon_derives; [apply derives_refl|].
+  apply sepcon_derives; [apply derives_refl|].
+  rewrite <- !sepcon_assoc, (sepcon_comm _ (ghost_set _ _)), !sepcon_assoc; apply sepcon_derives.
+  { match goal with |-?P |-- ?Q => replace P with Q; [apply derives_refl|] end.
+    f_equal; apply Extensionality_Ensembles.
+    constructor; intros ? X; unfold In in *.
+    - rewrite !app_nth, nth_repeat in X.
+      repeat destruct (lt_dec _ _); auto; try discriminate.
+      destruct (x - _)%nat; [|destruct n0]; inv X.
+    - destruct (lt_dec x (length lb)).
+      rewrite !app_nth, app_length.
+      destruct (lt_dec _ _); [|omega].
+      destruct (lt_dec _ _); [auto | omega].
+      { rewrite nth_overflow in X by omega; discriminate. } }
+  erewrite app_length, upto_app, iter_sepcon_app.
+  rewrite <- 2sepcon_assoc, (sepcon_comm _ (iter_sepcon _ _)), sepcon_assoc; apply sepcon_derives.
+  - eapply derives_trans with (_ * emp)%pred; [rewrite sepcon_emp; apply derives_refl|].
+    apply sepcon_derives.
+    + erewrite iter_sepcon_func_strong; auto.
+      intros ??%In_upto.
+      rewrite <- Zlength_correct in *.
+      rewrite <- !app_assoc, !app_Znth1 by (rewrite ?Zlength_app; omega); auto.
+    + rewrite iter_sepcon_emp'; auto.
+      intros ? Hin.
+      eapply in_map_iff in Hin as (? & ? & Hin%In_upto); subst.
+      rewrite <- Zlength_correct, Zlength_repeat in Hin.
+      rewrite <- Zlength_correct, <- app_assoc, app_Znth2 by omega.
+      erewrite app_Znth1 by (rewrite Zlength_repeat; omega).
+      unfold Znth; destruct (zlt _ _); auto.
+      rewrite nth_repeat; auto.
+  - unfold invariant.
+    rewrite emp_sepcon, !exp_sepcon2; apply exp_right with (length lg + i)%nat.
+    rewrite !exp_sepcon2; apply exp_right with g.
+    rewrite !sepcon_assoc; apply sepcon_derives; [apply derives_refl|].
+    rewrite sepcon_comm, sepcon_assoc; auto.
+Qed.
+
+(*Lemma wsat_open : forall i P,
+  (wsat * invariant i P * ghost_set g_en (Singleton _ i) |--
+  |==> wsat * |> P * ghost_list g_dis (list_singleton i (Some tt))).
+Proof.
+  intros; unfold wsat, invariant.
+  iIntros "((H & inv1) & en1)". iDestruct "H" as (l lg lb) "((((% & inv) & dis) & en) & I)". iDestruct "inv1" as (g) "[snap agree]".
+  iAssert (!! (i < length lg /\ Znth (Z.of_nat i) lg = g /\
+    exists b, Znth (Z.of_nat i) lb = Some b)%nat) as %Hi.
+  { iCombine "snap" "inv" as "inv"; unfold master_list; erewrite snap_master_join1.
+    iDestruct "inv" as "[% inv]".
+    apply list_incl_singleton in H0.
+    destruct (lt_dec i (length lg));
+      [|erewrite nth_overflow in H0 by (erewrite map_length, upto_length; omega); discriminate].
+    erewrite nth_map' with (d' := 0) in H0 by (rewrite upto_length; omega).
+    erewrite nth_upto in H0 by omega.
+    destruct (Znth (Z.of_nat i) lb); inv H0; iPureIntro; eauto. }
+  iMod (@own_dealloc (snap_PCM(ORD := list_order _)) with "snap").
+  iModIntro.
+  destruct Hi as (? & ? & b & Hi).
+  assert (nth i lb None = Some b) as Hi' by (rewrite <- nth_Znth in Hi; auto).
+  destruct b.
+  erewrite ghost_list_nth with (n := i) by (erewrite nth_map' with (d' := None), Hi'; eauto; omega).
+  iDestruct "dis" as "[token dis]".
+  erewrite iter_sepcon_Znth with (i0 := Z.of_nat i)
+    by (rewrite Zlength_upto; split; [|apply Nat2Z.inj_lt]; omega).
+  erewrite Znth_upto, Hi by omega.
+  iDestruct "I" as "((agree' & HP) & I)".
+  subst; iDestruct (agree_join with "[agree agree']") as "[imp agree]"; first iFrame.
+  iSplitR "token"; last auto.
+  iSplitR "HP imp"; last (iApply "imp"; auto).
+  iExists l, lg, (replace_nth i lb (Some false)).
+  rewrite replace_nth_length prop_true_andp; last auto.
+  iSplitR "I agree".
+  iSplitR "en en1".
+  iSplitR "dis".
+  - erewrite map_ext; eauto.
+    intros; simpl.
+    destruct (eq_dec a (Z.of_nat i)); [subst; rewrite Znth_replace_nth | rewrite Znth_replace_nth'];
+      auto; try omega.
+    rewrite Hi; auto.
+  - rewrite map_replace_nth; auto.
+  - iCombine "en en1" as "en"; erewrite ghost_set_join.
+    iDestruct "en" as "[% en]".
+    erewrite coPset_leibniz; auto; split.
+    + intros Hin%elem_of_union; rewrite -> elem_of_list_to_set, elem_of_list_In, in_map_iff in *; destruct Hin as [Hin | Hin].
+      * destruct Hin as (x' & ? & Hin); subst.
+        apply filter_In in Hin as [Hin ?].
+        do 2 eexists; eauto; apply filter_In; split; auto.
+        destruct (decide (x' = i)); [subst; rewrite nth_replace_nth | rewrite nth_replace_nth']; auto; omega.
+      * apply elem_of_singleton in Hin; subst.
+        do 2 eexists; eauto; apply filter_In.
+        split; [|rewrite nth_replace_nth; auto; omega].
+        apply in_seq; omega.
+    + intros Hin; rewrite elem_of_union; rewrite -> elem_of_list_to_set, elem_of_list_In, in_map_iff in *.
+      destruct Hin as (x' & ? & Hin); subst.
+      destruct (decide (x' = i)); [subst; rewrite elem_of_singleton; auto|].
+      left; do 2 eexists; eauto.
+      apply filter_In in Hin as [Hin ?]; rewrite filter_In; split; auto.
+      erewrite nth_replace_nth' in H2; auto.
+  - erewrite iter_sepcon_Znth with (i0 := Z.of_nat i)(l0 := upto _)
+      by (rewrite Zlength_upto; split; [|apply Nat2Z.inj_lt]; omega).
+    erewrite Znth_upto, Znth_replace_nth by omega; iFrame.
+    erewrite iter_sepcon_func_strong; auto.
+    unfold remove_Znth; intros ? Hin.
+    rewrite Znth_replace_nth'; auto.
+    intro; subst.
+    apply in_app in Hin as [?%In_sublist_upto | ?%In_sublist_upto]; omega.
+  - iCombine "en en1" as "en"; erewrite ghost_set_join.
+    iDestruct "en" as "[% en]".
+    rewrite -> elem_of_disjoint in H2.
+    contradiction (H2 (Pos.of_nat (S i))).
+    + rewrite -> elem_of_list_to_set, elem_of_list_In, in_map_iff.
+      do 2 eexists; eauto.
+      rewrite filter_In; split; [|rewrite Hi'; auto].
+      apply in_seq; omega.
+    + apply elem_of_singleton; auto.
+Qed.
+
+(* up *)
+Lemma replace_nth_same' : forall {A} n l (a d : A), nth n l d = a -> replace_nth n l a = l.
+Proof.
+  intros; subst; apply replace_nth_same.
+Qed.
+
+Lemma wsat_close : forall i P,
+  (wsat * invariant i P * |> P * ghost_list g_dis (list_singleton i (Some tt)) |--
+  |==> wsat * ghost_set g_en (base.singleton (Pos.of_nat (S i))))%I.
+Proof.
+  intros; unfold wsat, invariant.
+  iIntros "(((H & inv1) & HP) & dis1)". iDestruct "H" as (l lg lb) "((((% & inv) & dis) & en) & I)". iDestruct "inv1" as (g) "[snap agree]".
+  iAssert (!!(i < length lg /\ Znth (Z.of_nat i) lg = g /\
+    exists b, Znth (Z.of_nat i) lb = Some b)%nat) as %Hi.
+  { iCombine "snap inv" as "inv"; unfold master_list; erewrite snap_master_join1.
+    iDestruct "inv" as "[% inv]".
+    apply list_incl_singleton in H0.
+    destruct (lt_dec i (length lg));
+      [|erewrite nth_overflow in H0 by (erewrite map_length, upto_length; omega); discriminate].
+    erewrite nth_map' with (d' := 0) in H0 by (rewrite upto_length; omega).
+    erewrite nth_upto in H0 by omega.
+    destruct (Znth (Z.of_nat i) lb); inv H0; eauto. }
+  iMod (@own_dealloc (snap_PCM(ORD := list_order _)) with "snap").
+  iModIntro.
+  destruct Hi as (? & ? & b & Hi).
+  assert (nth i lb None = Some b) as Hi' by (rewrite <- nth_Znth in Hi; auto).
+  destruct b.
+  { iCombine "dis dis1" as "dis".
+    iDestruct (own_valid_2(RA := list_PCM _) with "dis") as %H2.
+    destruct H2 as (? & J & _).
+    apply list_join_nth with (n := i) in J.
+    erewrite nth_singleton, nth_map' with (d' := None) in J by omega.
+    rewrite Hi' in J; inv J.
+    inv H5.
+    inv H3. }
+  erewrite ghost_set_remove with (a := Pos.of_nat (S i)).
+  iDestruct "en" as "[$ en]".
+  iExists l, lg, (replace_nth i lb (Some true)).
+  rewrite replace_nth_length prop_true_andp; last auto.
+  iSplitR "I agree HP".
+  iSplitR "en".
+  iSplitR "dis dis1".
+  - erewrite map_ext; eauto.
+    intros.
+    destruct (eq_dec a (Z.of_nat i)); [subst; rewrite Znth_replace_nth | rewrite Znth_replace_nth'];
+      auto; try omega.
+    rewrite Hi; auto.
+  - iCombine "dis1 dis" as "dis"; setoid_rewrite <- own_op; auto.
+    rewrite map_replace_nth.
+    apply (list_join_singleton(P := token_PCM)).
+    { rewrite map_length; omega. }
+    erewrite nth_map' with (d' := None) by omega.
+    rewrite Hi'; constructor.
+  - erewrite coPset_leibniz; auto; split.
+    + rewrite -> elem_of_difference, !elem_of_list_to_set, !elem_of_list_In, !in_map_iff.
+      intros ((? & ? & Hin) & Hout); subst.
+      do 2 eexists; eauto.
+      rewrite -> filter_In in *; destruct Hin; split; auto.
+      rewrite nth_replace_nth'; auto.
+      intro; subst; contradiction Hout; apply elem_of_singleton; auto.
+    + rewrite -> elem_of_difference, !elem_of_list_to_set, !elem_of_list_In, !in_map_iff.
+      intros (x' & ? & Hin) ; subst.
+      rewrite -> filter_In in *; destruct Hin as [? Hin].
+      destruct (decide (x' = i)); [subst; erewrite nth_replace_nth in Hin by omega; discriminate|].
+      erewrite nth_replace_nth' in Hin by auto.
+      split; [|rewrite elem_of_singleton; auto].
+      do 2 eexists; eauto.
+      rewrite filter_In; split; auto.
+      intros X%Nat2Pos.inj; congruence.
+  - erewrite iter_sepcon_Znth with (i0 := Z.of_nat i)
+      by (rewrite Zlength_upto; split; [|apply Nat2Z.inj_lt]; omega).
+    erewrite iter_sepcon_Znth with (i0 := Z.of_nat i)(l0 := upto _)
+      by (rewrite Zlength_upto; split; [|apply Nat2Z.inj_lt]; omega).
+    erewrite !Znth_upto, !Znth_replace_nth by omega.
+    rewrite Hi.
+    iDestruct "I" as "[agree' I]".
+    subst; iDestruct (agree_join2 with "[agree' agree]") as "[imp agree]"; first iFrame.
+    iPoseProof ("imp" with "HP") as "?"; iFrame.
+    erewrite iter_sepcon_func_strong; eauto.
+    unfold remove_Znth; intros ? Hin.
+    rewrite Znth_replace_nth'; auto.
+    intro; subst.
+    apply in_app in Hin as [?%In_sublist_upto | ?%In_sublist_upto]; omega.
+  - rewrite -> elem_of_list_to_set, elem_of_list_In, in_map_iff.
+    do 2 eexists; eauto.
+    rewrite filter_In; split; [|rewrite Hi'; auto].
+    apply in_seq; omega.
+Qed.*)
+
+Lemma invariant_dealloc : forall i P, invariant i P |-- |==> emp.
+Proof.
+  intros; unfold invariant.
+  apply exp_left; intro g.
+  rewrite <- (emp_sepcon emp).
+  eapply derives_trans.
+  apply sepcon_derives; apply ghost_dealloc.
+  { eapply derives_trans, bupd_trans.
+    eapply derives_trans; [apply bupd_frame_r | apply bupd_mono, bupd_frame_l]. }
+Qed.
+
+Lemma invariant_super_non_expansive : forall n N P,
+  approx n (invariant N P) = approx n (invariant N (approx n P)).
+Proof.
+  intros; unfold invariant.
+  rewrite !approx_exp; f_equal; extensionality g.
+  rewrite !approx_sepcon; f_equal.
+  apply own_super_non_expansive.
+Qed.
+
+(* Consider putting rules for invariants and fancy updates in msl (a la ghost_seplog), and proofs
+   in veric (a la own). *)
+
+Lemma ghost_set_empty : forall g s,
+  (ghost_set g s = ghost_set g s * ghost_set g (Empty_set _))%pred.
+Proof.
+  intros.
+  apply ghost_op.
+  hnf; split.
+  - constructor.
+    intros ? X; inv X.
+    inv H0.
+  - apply Extensionality_Ensembles.
+    constructor; intros ? X; [left | inv X]; auto.
+    inv H.
+Qed.
+
+Lemma wsat_empty_eq : (wsat = wsat * ghost_set g_en (Empty_set _))%pred.
+Proof.
+  unfold wsat.
+  repeat (rewrite exp_sepcon1; f_equal; extensionality).
+  rewrite !sepcon_andp_prop1; f_equal.
+  rewrite !sepcon_assoc; f_equal; f_equal.
+  rewrite !(sepcon_comm (ghost_set _ _)), sepcon_assoc; f_equal.
+  rewrite sepcon_comm; apply ghost_set_empty.
+Qed.
+
+End Invariants.
+
+(*Lemma make_wsat : (emp |-- |==> EX inv_names : invG, wsat)%I.
+Proof.
+  unfold wsat.
+  iIntros.
+  iMod (own_alloc(RA := snap_PCM(ORD := list_order gname)) (Tsh, nil) NoneP with "[$]") as (g_inv) "inv"; first (simpl; auto).
+  iMod (own_alloc(RA := list_PCM (exclusive_PCM unit)) nil NoneP with "[$]") as (g_dis) "dis"; first (simpl; auto).
+  iMod (own_alloc(RA := set_PCM) empty NoneP with "[$]") as (g_en) "en"; first (simpl; auto).
+  iModIntro.
+  iExists {| g_inv := g_inv; g_dis := g_dis; g_en := g_en |}.
+  iExists nil, nil, nil; simpl; iFrame; auto.
+Qed.*)
